ETCS_Exp.thy
@@ -206,7 +206,7 @@ proof -
   have "n ^\<^sub>\<nat> (successor \<circ>\<^sub>c zero) =  eval_func  \<nat>\<^sub>c \<nat>\<^sub>c \<circ>\<^sub>c \<langle>n, exp_curried \<circ>\<^sub>c(successor \<circ>\<^sub>c zero) \<rangle>"
     using assms comp_type exp_def2 successor_type zero_type by blast
   also have "... = eval_func  \<nat>\<^sub>c \<nat>\<^sub>c \<circ>\<^sub>c \<langle>n, ((mult2 \<circ>\<^sub>c\<langle>left_cart_proj \<nat>\<^sub>c (\<nat>\<^sub>c\<^bsup>\<nat>\<^sub>c\<^esup>),eval_func \<nat>\<^sub>c \<nat>\<^sub>c\<rangle>)\<^sup>\<sharp>) \<circ>\<^sub>cexp_curried \<circ>\<^sub>c zero \<rangle>"
-    using assms comp_associative2 exp_curried_comp_succ_eq exp_curried_type mult_pie_sharp_type successor_type zero_type by auto 
+    using assms by (typecheck_cfuncs, simp add: cfunc_type_def comp_associative exp_curried_comp_succ_eq)
   also have "... = eval_func  \<nat>\<^sub>c \<nat>\<^sub>c \<circ>\<^sub>c \<langle>n, ((mult2 \<circ>\<^sub>c\<langle>left_cart_proj \<nat>\<^sub>c (\<nat>\<^sub>c\<^bsup>\<nat>\<^sub>c\<^esup>),eval_func \<nat>\<^sub>c \<nat>\<^sub>c\<rangle>)\<^sup>\<sharp>) \<circ>\<^sub>c ((successor \<circ>\<^sub>c zero \<circ>\<^sub>c right_cart_proj \<nat>\<^sub>c one)\<^sup>\<sharp>)\<rangle>"
     by (simp add: exp_curried_0_eq)
   also have "... = eval_func  \<nat>\<^sub>c \<nat>\<^sub>c \<circ>\<^sub>c \<langle>id\<^sub>c \<nat>\<^sub>c \<circ>\<^sub>c n, ((mult2 \<circ>\<^sub>c\<langle>left_cart_proj \<nat>\<^sub>c (\<nat>\<^sub>c\<^bsup>\<nat>\<^sub>c\<^esup>),eval_func \<nat>\<^sub>c \<nat>\<^sub>c\<rangle>)\<^sup>\<sharp>) \<circ>\<^sub>c ((successor \<circ>\<^sub>c zero \<circ>\<^sub>c right_cart_proj \<nat>\<^sub>c one)\<^sup>\<sharp>)\<rangle>"
