ETCS_Mult.thy
@@ -1524,7 +1524,7 @@ proof -
     using transpose_func_type by blast
   have id_multmultidsharp_type: "(id\<^sub>c (\<nat>\<^sub>c\<times>\<^sub>c\<nat>\<^sub>c) \<times>\<^sub>f ((mult2 \<circ>\<^sub>c (mult2 \<times>\<^sub>f id\<^sub>c \<nat>\<^sub>c))\<^sup>\<sharp>)): (\<nat>\<^sub>c\<times>\<^sub>c\<nat>\<^sub>c) \<times>\<^sub>c \<nat>\<^sub>c \<rightarrow> (\<nat>\<^sub>c\<times>\<^sub>c\<nat>\<^sub>c) \<times>\<^sub>c \<nat>\<^sub>c\<^bsup>(\<nat>\<^sub>c\<times>\<^sub>c \<nat>\<^sub>c)\<^esup>"
     by (meson cfunc_cross_prod_type id_type multmultIdSharp_type)
-  
+ 
   
   have main_result: "(mult2 \<circ>\<^sub>c (mult2 \<times>\<^sub>f id\<^sub>c \<nat>\<^sub>c))\<^sup>\<sharp> = 
 (mult2 \<circ>\<^sub>c (id\<^sub>c \<nat>\<^sub>c  \<times>\<^sub>f mult2) \<circ>\<^sub>c \<langle>(left_cart_proj \<nat>\<^sub>c \<nat>\<^sub>c) \<circ>\<^sub>c (left_cart_proj (\<nat>\<^sub>c\<times>\<^sub>c \<nat>\<^sub>c) \<nat>\<^sub>c),
@@ -1567,429 +1567,456 @@ proof -
               using cart_prod_decomp x_def by blast
             have y1_type: "x = \<langle>\<langle>p,q\<rangle>, id one\<rangle>"
               by (simp add: x_def y_def)
+            have y_type: "\<langle>p,q\<rangle> \<in>\<^sub>c (\<nat>\<^sub>c \<times>\<^sub>c \<nat>\<^sub>c)"
+              using x_def y_def by blast
+            have pq0_type: "\<langle>\<langle>p,q\<rangle>,zero\<rangle> \<in>\<^sub>c (\<nat>\<^sub>c \<times>\<^sub>c \<nat>\<^sub>c) \<times>\<^sub>c \<nat>\<^sub>c"
+              by (simp add: cfunc_prod_type y_type zero_type)
+            
 
             have "(eval_func \<nat>\<^sub>c (\<nat>\<^sub>c \<times>\<^sub>c \<nat>\<^sub>c) \<circ>\<^sub>c
           id\<^sub>c (\<nat>\<^sub>c \<times>\<^sub>c \<nat>\<^sub>c) \<times>\<^sub>f (mult2 \<circ>\<^sub>c mult2 \<times>\<^sub>f id\<^sub>c \<nat>\<^sub>c)\<^sup>\<sharp> \<circ>\<^sub>c zero) \<circ>\<^sub>c x = 
             (((eval_func \<nat>\<^sub>c (\<nat>\<^sub>c \<times>\<^sub>c \<nat>\<^sub>c) \<circ>\<^sub>c
           id\<^sub>c (\<nat>\<^sub>c \<times>\<^sub>c \<nat>\<^sub>c) \<times>\<^sub>f (mult2 \<circ>\<^sub>c mult2 \<times>\<^sub>f id\<^sub>c \<nat>\<^sub>c)\<^sup>\<sharp>)) \<circ>\<^sub>c (id\<^sub>c (\<nat>\<^sub>c \<times>\<^sub>c \<nat>\<^sub>c) \<times>\<^sub>f  zero)) \<circ>\<^sub>c x"
-              
-
-
-(*
-  have f1: "((eval_func \<nat>\<^sub>c (\<nat>\<^sub>c\<times>\<^sub>c\<nat>\<^sub>c))\<circ>\<^sub>c
-(id\<^sub>c (\<nat>\<^sub>c\<times>\<^sub>c\<nat>\<^sub>c) \<times>\<^sub>f ((mult2 \<circ>\<^sub>c (mult2 \<times>\<^sub>f id\<^sub>c \<nat>\<^sub>c))\<^sup>\<sharp>\<circ>\<^sub>c zero)))\<circ>\<^sub>c \<langle>\<langle>a,b\<rangle>,id\<^sub>c one\<rangle> = zero" 
-  proof - 
-    have "((eval_func \<nat>\<^sub>c (\<nat>\<^sub>c\<times>\<^sub>c\<nat>\<^sub>c))\<circ>\<^sub>c 
-(id\<^sub>c (\<nat>\<^sub>c\<times>\<^sub>c\<nat>\<^sub>c) \<times>\<^sub>f ((mult2 \<circ>\<^sub>c (mult2 \<times>\<^sub>f id\<^sub>c \<nat>\<^sub>c))\<^sup>\<sharp>\<circ>\<^sub>c zero)))\<circ>\<^sub>c \<langle>\<langle>a,b\<rangle>,id\<^sub>c one\<rangle> = 
-(eval_func \<nat>\<^sub>c (\<nat>\<^sub>c\<times>\<^sub>c\<nat>\<^sub>c))\<circ>\<^sub>c 
-(id\<^sub>c (\<nat>\<^sub>c\<times>\<^sub>c\<nat>\<^sub>c) \<times>\<^sub>f ((mult2 \<circ>\<^sub>c (mult2 \<times>\<^sub>f id\<^sub>c \<nat>\<^sub>c))\<^sup>\<sharp>\<circ>\<^sub>c zero))\<circ>\<^sub>c \<langle>\<langle>a,b\<rangle>,id\<^sub>c one\<rangle>"
-    using assms by (typecheck_cfuncs, simp add: comp_associative2)
-   also have "... = (eval_func \<nat>\<^sub>c (\<nat>\<^sub>c\<times>\<^sub>c\<nat>\<^sub>c))\<circ>\<^sub>c 
-(id\<^sub>c (\<nat>\<^sub>c\<times>\<^sub>c\<nat>\<^sub>c) \<times>\<^sub>f ((mult2 \<circ>\<^sub>c (mult2 \<times>\<^sub>f id\<^sub>c \<nat>\<^sub>c))\<^sup>\<sharp>))\<circ>\<^sub>c ((id\<^sub>c (\<nat>\<^sub>c\<times>\<^sub>c\<nat>\<^sub>c) \<times>\<^sub>f zero)) \<circ>\<^sub>c \<langle>\<langle>a,b\<rangle>,id\<^sub>c one\<rangle>"
-        using assms by (typecheck_cfuncs, smt comp_associative2 flat_cancels_sharp inv_transpose_func_def2 inv_transpose_of_composition)
-    also have "... = (mult2 \<circ>\<^sub>c (mult2 \<times>\<^sub>f id\<^sub>c \<nat>\<^sub>c)) \<circ>\<^sub>c   \<langle> id\<^sub>c (\<nat>\<^sub>c\<times>\<^sub>c\<nat>\<^sub>c) \<circ>\<^sub>c \<langle>a,b\<rangle>, zero \<circ>\<^sub>c id\<^sub>c one\<rangle>"
-        using assms by (typecheck_cfuncs, smt cfunc_cross_prod_comp_cfunc_prod comp_associative2 transpose_func_def)
-    also have "... = mult2 \<circ>\<^sub>c (mult2 \<times>\<^sub>f id\<^sub>c \<nat>\<^sub>c)  \<circ>\<^sub>c   \<langle>\<langle>a,b\<rangle>, zero\<rangle>"
-        using assms by (typecheck_cfuncs, simp add: comp_associative2 id_left_unit2 id_right_unit2)
-    also have "... = mult2 \<circ>\<^sub>c \<langle>mult2 \<circ>\<^sub>c \<langle>a,b\<rangle>, zero\<rangle> "
-      using ab_type cfunc_cross_prod_comp_cfunc_prod id_left_unit2 id_type mult2_type zero_type by fastforce
-    also have "... = zero"
-      using mult_def mult_respects_zero_right multab_type by auto
-then show ?thesis using calculation by auto
-qed
-
-
-  have f2: "((eval_func \<nat>\<^sub>c (\<nat>\<^sub>c\<times>\<^sub>c\<nat>\<^sub>c))\<circ>\<^sub>c 
+              by (typecheck_cfuncs, metis inv_transpose_func_def2 inv_transpose_of_composition)
+            also have "... = ((eval_func \<nat>\<^sub>c (\<nat>\<^sub>c \<times>\<^sub>c \<nat>\<^sub>c) \<circ>\<^sub>c
+          id\<^sub>c (\<nat>\<^sub>c \<times>\<^sub>c \<nat>\<^sub>c) \<times>\<^sub>f (mult2 \<circ>\<^sub>c mult2 \<times>\<^sub>f id\<^sub>c \<nat>\<^sub>c)\<^sup>\<sharp>)) \<circ>\<^sub>c (id\<^sub>c (\<nat>\<^sub>c \<times>\<^sub>c \<nat>\<^sub>c) \<times>\<^sub>f  zero) \<circ>\<^sub>c x"
+              using comp_associative2 x_type by (typecheck_cfuncs, auto)
+            also have "... = (mult2 \<circ>\<^sub>c mult2 \<times>\<^sub>f id\<^sub>c \<nat>\<^sub>c) \<circ>\<^sub>c ((id\<^sub>c (\<nat>\<^sub>c \<times>\<^sub>c \<nat>\<^sub>c) \<times>\<^sub>f  zero) \<circ>\<^sub>c x)"
+              using multmultId_type transpose_func_def by (typecheck_cfuncs, auto)
+            also have "... = (mult2 \<circ>\<^sub>c mult2 \<times>\<^sub>f id\<^sub>c \<nat>\<^sub>c) \<circ>\<^sub>c ((id\<^sub>c (\<nat>\<^sub>c \<times>\<^sub>c \<nat>\<^sub>c) \<times>\<^sub>f  zero) \<circ>\<^sub>c \<langle>\<langle>p,q\<rangle>, id one\<rangle>)"
+              by (simp add: y1_type)
+            also have "... = (mult2 \<circ>\<^sub>c mult2 \<times>\<^sub>f id\<^sub>c \<nat>\<^sub>c) \<circ>\<^sub>c  \<langle>id\<^sub>c (\<nat>\<^sub>c \<times>\<^sub>c \<nat>\<^sub>c)\<circ>\<^sub>c \<langle>p,q\<rangle>,zero \<circ>\<^sub>c id one\<rangle>"
+              by (typecheck_cfuncs, smt cfunc_cross_prod_comp_cfunc_prod y_def)
+            also have "... = (mult2 \<circ>\<^sub>c (mult2 \<times>\<^sub>f id\<^sub>c \<nat>\<^sub>c)) \<circ>\<^sub>c  \<langle>\<langle>p,q\<rangle>,zero\<rangle>"
+              by (typecheck_cfuncs, metis id_left_unit2 id_right_unit2 y_def)
+            also have "... = mult2 \<circ>\<^sub>c ((mult2 \<times>\<^sub>f id\<^sub>c \<nat>\<^sub>c) \<circ>\<^sub>c  \<langle>\<langle>p,q\<rangle>,zero\<rangle>)"
+              using comp_associative2 pq0_type by (typecheck_cfuncs, auto)
+            also have "... = mult2 \<circ>\<^sub>c   \<langle>mult2\<circ>\<^sub>c \<langle>p,q\<rangle>,id\<^sub>c \<nat>\<^sub>c\<circ>\<^sub>c zero\<rangle>"
+              using cfunc_cross_prod_comp_cfunc_prod y_type by (typecheck_cfuncs, auto)
+            also have "... = (mult2\<circ>\<^sub>c \<langle>p,q\<rangle>) \<cdot>\<^sub>\<nat> zero"
+              using id_left_unit2 mult_def zero_type by auto
+            also have "... = zero"
+              using comp_type mult2_type mult_respects_zero_right y_type by blast
+            also have "... = mult2 \<circ>\<^sub>c  \<langle>id\<^sub>c \<nat>\<^sub>c \<circ>\<^sub>c p ,mult2 \<circ>\<^sub>c \<langle>q,zero\<rangle>  \<rangle>"
+              using mult_def mult_respects_zero_right y_def by (typecheck_cfuncs, presburger)
+            also have "... = mult2 \<circ>\<^sub>c (id\<^sub>c \<nat>\<^sub>c  \<times>\<^sub>f mult2) \<circ>\<^sub>c \<langle>p , \<langle>q,zero\<rangle>  \<rangle>"
+              by (typecheck_cfuncs , smt cfunc_cross_prod_comp_cfunc_prod y_def)
+            also have "... = mult2 \<circ>\<^sub>c (id\<^sub>c \<nat>\<^sub>c  \<times>\<^sub>f mult2) \<circ>\<^sub>c \<langle>(left_cart_proj \<nat>\<^sub>c \<nat>\<^sub>c) \<circ>\<^sub>c  \<langle>p,q\<rangle>,
+                             \<langle>(right_cart_proj \<nat>\<^sub>c \<nat>\<^sub>c) \<circ>\<^sub>c  \<langle>p,q\<rangle>  ,zero  \<rangle>  \<rangle>"
+              by (typecheck_cfuncs, metis left_cart_proj_cfunc_prod right_cart_proj_cfunc_prod y_def)
+            also have "... = mult2 \<circ>\<^sub>c (id\<^sub>c \<nat>\<^sub>c  \<times>\<^sub>f mult2) \<circ>\<^sub>c \<langle>(left_cart_proj \<nat>\<^sub>c \<nat>\<^sub>c) \<circ>\<^sub>c (left_cart_proj (\<nat>\<^sub>c\<times>\<^sub>c \<nat>\<^sub>c) \<nat>\<^sub>c) \<circ>\<^sub>c \<langle>\<langle>p,q\<rangle>,zero\<rangle>,
+  \<langle>(right_cart_proj \<nat>\<^sub>c \<nat>\<^sub>c) \<circ>\<^sub>c (left_cart_proj (\<nat>\<^sub>c\<times>\<^sub>c \<nat>\<^sub>c) \<nat>\<^sub>c) \<circ>\<^sub>c \<langle>\<langle>p,q\<rangle>,zero\<rangle>  , (right_cart_proj (\<nat>\<^sub>c\<times>\<^sub>c \<nat>\<^sub>c) \<nat>\<^sub>c) \<circ>\<^sub>c \<langle>\<langle>p,q\<rangle>,zero\<rangle>  \<rangle>  \<rangle>"
+              using left_cart_proj_cfunc_prod right_cart_proj_cfunc_prod y_type by (typecheck_cfuncs, auto)
+            also have "... = mult2 \<circ>\<^sub>c (id\<^sub>c \<nat>\<^sub>c  \<times>\<^sub>f mult2) \<circ>\<^sub>c \<langle>(left_cart_proj \<nat>\<^sub>c \<nat>\<^sub>c) \<circ>\<^sub>c (left_cart_proj (\<nat>\<^sub>c\<times>\<^sub>c \<nat>\<^sub>c) \<nat>\<^sub>c) \<circ>\<^sub>c \<langle>\<langle>p,q\<rangle>,zero\<rangle>,
+\<langle>(right_cart_proj \<nat>\<^sub>c \<nat>\<^sub>c) \<circ>\<^sub>c (left_cart_proj (\<nat>\<^sub>c\<times>\<^sub>c \<nat>\<^sub>c) \<nat>\<^sub>c), (right_cart_proj (\<nat>\<^sub>c\<times>\<^sub>c \<nat>\<^sub>c) \<nat>\<^sub>c)\<rangle> \<circ>\<^sub>c \<langle>\<langle>p,q\<rangle>,zero\<rangle>  \<rangle>"
+              using cfunc_prod_comp comp_associative2 pq0_type by (typecheck_cfuncs, auto)  
+            also have "... = mult2 \<circ>\<^sub>c (id\<^sub>c \<nat>\<^sub>c  \<times>\<^sub>f mult2) \<circ>\<^sub>c \<langle>(left_cart_proj \<nat>\<^sub>c \<nat>\<^sub>c) \<circ>\<^sub>c (left_cart_proj (\<nat>\<^sub>c\<times>\<^sub>c \<nat>\<^sub>c) \<nat>\<^sub>c),
+\<langle>(right_cart_proj \<nat>\<^sub>c \<nat>\<^sub>c) \<circ>\<^sub>c (left_cart_proj (\<nat>\<^sub>c\<times>\<^sub>c \<nat>\<^sub>c) \<nat>\<^sub>c), (right_cart_proj (\<nat>\<^sub>c\<times>\<^sub>c \<nat>\<^sub>c) \<nat>\<^sub>c)\<rangle>\<rangle>\<circ>\<^sub>c \<langle>\<langle>p,q\<rangle>,zero\<rangle>"
+              using cfunc_prod_comp comp_associative2 pq0_type by (typecheck_cfuncs, auto)
+             also have "... = mult2 \<circ>\<^sub>c (id\<^sub>c \<nat>\<^sub>c  \<times>\<^sub>f mult2) \<circ>\<^sub>c \<langle>(left_cart_proj \<nat>\<^sub>c \<nat>\<^sub>c) \<circ>\<^sub>c (left_cart_proj (\<nat>\<^sub>c\<times>\<^sub>c \<nat>\<^sub>c) \<nat>\<^sub>c),
+\<langle>(right_cart_proj \<nat>\<^sub>c \<nat>\<^sub>c) \<circ>\<^sub>c (left_cart_proj (\<nat>\<^sub>c\<times>\<^sub>c \<nat>\<^sub>c) \<nat>\<^sub>c), (right_cart_proj (\<nat>\<^sub>c\<times>\<^sub>c \<nat>\<^sub>c) \<nat>\<^sub>c)\<rangle>\<rangle>\<circ>\<^sub>c \<langle>id\<^sub>c (\<nat>\<^sub>c\<times>\<^sub>c\<nat>\<^sub>c) \<circ>\<^sub>c \<langle>p,q\<rangle>,zero \<circ>\<^sub>cid\<^sub>c one\<rangle>"
+               using id_left_unit2 id_right_unit2 y_type by (typecheck_cfuncs, auto)
+            also have "... = (mult2 \<circ>\<^sub>c (id\<^sub>c \<nat>\<^sub>c  \<times>\<^sub>f mult2) \<circ>\<^sub>c \<langle>(left_cart_proj \<nat>\<^sub>c \<nat>\<^sub>c) \<circ>\<^sub>c (left_cart_proj (\<nat>\<^sub>c\<times>\<^sub>c \<nat>\<^sub>c) \<nat>\<^sub>c),
+    \<langle>(right_cart_proj \<nat>\<^sub>c \<nat>\<^sub>c) \<circ>\<^sub>c (left_cart_proj (\<nat>\<^sub>c\<times>\<^sub>c \<nat>\<^sub>c) \<nat>\<^sub>c), (right_cart_proj (\<nat>\<^sub>c\<times>\<^sub>c \<nat>\<^sub>c) \<nat>\<^sub>c)\<rangle>\<rangle>)\<circ>\<^sub>c (id\<^sub>c (\<nat>\<^sub>c\<times>\<^sub>c\<nat>\<^sub>c) \<times>\<^sub>f zero)  \<circ>\<^sub>c \<langle>\<langle>p,q\<rangle>,id\<^sub>c one\<rangle>"
+              by (typecheck_cfuncs, smt cfunc_cross_prod_comp_cfunc_prod comp_associative2 y_type)       
+            also have "... = (eval_func \<nat>\<^sub>c (\<nat>\<^sub>c\<times>\<^sub>c\<nat>\<^sub>c))\<circ>\<^sub>c 
+    (id\<^sub>c (\<nat>\<^sub>c\<times>\<^sub>c\<nat>\<^sub>c) \<times>\<^sub>f ((mult2 \<circ>\<^sub>c (id\<^sub>c \<nat>\<^sub>c  \<times>\<^sub>f mult2) \<circ>\<^sub>c \<langle>(left_cart_proj \<nat>\<^sub>c \<nat>\<^sub>c) \<circ>\<^sub>c (left_cart_proj (\<nat>\<^sub>c\<times>\<^sub>c \<nat>\<^sub>c) \<nat>\<^sub>c),
+    \<langle>(right_cart_proj \<nat>\<^sub>c \<nat>\<^sub>c) \<circ>\<^sub>c (left_cart_proj (\<nat>\<^sub>c\<times>\<^sub>c \<nat>\<^sub>c) \<nat>\<^sub>c), (right_cart_proj (\<nat>\<^sub>c\<times>\<^sub>c \<nat>\<^sub>c) \<nat>\<^sub>c)\<rangle>\<rangle>)\<^sup>\<sharp> )) \<circ>\<^sub>c (id\<^sub>c (\<nat>\<^sub>c\<times>\<^sub>c\<nat>\<^sub>c) \<times>\<^sub>f zero)  \<circ>\<^sub>c \<langle>\<langle>p,q\<rangle>,id\<^sub>c one\<rangle>"
+              by (typecheck_cfuncs , smt cfunc_type_def comp_associative transpose_func_def y_type)        
+            also have "... = (eval_func \<nat>\<^sub>c (\<nat>\<^sub>c\<times>\<^sub>c\<nat>\<^sub>c))\<circ>\<^sub>c 
 (id\<^sub>c (\<nat>\<^sub>c\<times>\<^sub>c\<nat>\<^sub>c) \<times>\<^sub>f ((mult2 \<circ>\<^sub>c (id\<^sub>c \<nat>\<^sub>c  \<times>\<^sub>f mult2) \<circ>\<^sub>c \<langle>(left_cart_proj \<nat>\<^sub>c \<nat>\<^sub>c) \<circ>\<^sub>c (left_cart_proj (\<nat>\<^sub>c\<times>\<^sub>c \<nat>\<^sub>c) \<nat>\<^sub>c),
-\<langle>(right_cart_proj \<nat>\<^sub>c \<nat>\<^sub>c) \<circ>\<^sub>c (left_cart_proj (\<nat>\<^sub>c\<times>\<^sub>c \<nat>\<^sub>c) \<nat>\<^sub>c), (right_cart_proj (\<nat>\<^sub>c\<times>\<^sub>c \<nat>\<^sub>c) \<nat>\<^sub>c)\<rangle>\<rangle>)\<^sup>\<sharp> \<circ>\<^sub>c zero))) \<circ>\<^sub>c \<langle>\<langle>a,b\<rangle>,id\<^sub>c one\<rangle> = zero" 
-  proof - 
-    have "((eval_func \<nat>\<^sub>c (\<nat>\<^sub>c\<times>\<^sub>c\<nat>\<^sub>c))\<circ>\<^sub>c 
+\<langle>(right_cart_proj \<nat>\<^sub>c \<nat>\<^sub>c) \<circ>\<^sub>c (left_cart_proj (\<nat>\<^sub>c\<times>\<^sub>c \<nat>\<^sub>c) \<nat>\<^sub>c), (right_cart_proj (\<nat>\<^sub>c\<times>\<^sub>c \<nat>\<^sub>c) \<nat>\<^sub>c)\<rangle>\<rangle>)\<^sup>\<sharp> \<circ>\<^sub>c zero)) \<circ>\<^sub>c \<langle>\<langle>p,q\<rangle>,id\<^sub>c one\<rangle>"
+              by (typecheck_cfuncs, smt comp_associative2 inv_transpose_func_def2 inv_transpose_of_composition transpose_func_def x_type y1_type)        
+            also have "... = ((eval_func \<nat>\<^sub>c (\<nat>\<^sub>c\<times>\<^sub>c\<nat>\<^sub>c))\<circ>\<^sub>c 
 (id\<^sub>c (\<nat>\<^sub>c\<times>\<^sub>c\<nat>\<^sub>c) \<times>\<^sub>f ((mult2 \<circ>\<^sub>c (id\<^sub>c \<nat>\<^sub>c  \<times>\<^sub>f mult2) \<circ>\<^sub>c \<langle>(left_cart_proj \<nat>\<^sub>c \<nat>\<^sub>c) \<circ>\<^sub>c (left_cart_proj (\<nat>\<^sub>c\<times>\<^sub>c \<nat>\<^sub>c) \<nat>\<^sub>c),
-\<langle>(right_cart_proj \<nat>\<^sub>c \<nat>\<^sub>c) \<circ>\<^sub>c (left_cart_proj (\<nat>\<^sub>c\<times>\<^sub>c \<nat>\<^sub>c) \<nat>\<^sub>c), (right_cart_proj (\<nat>\<^sub>c\<times>\<^sub>c \<nat>\<^sub>c) \<nat>\<^sub>c)\<rangle>\<rangle>)\<^sup>\<sharp> \<circ>\<^sub>c zero))) \<circ>\<^sub>c \<langle>\<langle>a,b\<rangle>,id\<^sub>c one\<rangle> = 
-   (eval_func \<nat>\<^sub>c (\<nat>\<^sub>c\<times>\<^sub>c\<nat>\<^sub>c))\<circ>\<^sub>c 
-(id\<^sub>c (\<nat>\<^sub>c\<times>\<^sub>c\<nat>\<^sub>c) \<times>\<^sub>f ((mult2 \<circ>\<^sub>c (id\<^sub>c \<nat>\<^sub>c  \<times>\<^sub>f mult2) \<circ>\<^sub>c \<langle>(left_cart_proj \<nat>\<^sub>c \<nat>\<^sub>c) \<circ>\<^sub>c (left_cart_proj (\<nat>\<^sub>c\<times>\<^sub>c \<nat>\<^sub>c) \<nat>\<^sub>c),
-\<langle>(right_cart_proj \<nat>\<^sub>c \<nat>\<^sub>c) \<circ>\<^sub>c (left_cart_proj (\<nat>\<^sub>c\<times>\<^sub>c \<nat>\<^sub>c) \<nat>\<^sub>c), (right_cart_proj (\<nat>\<^sub>c\<times>\<^sub>c \<nat>\<^sub>c) \<nat>\<^sub>c)\<rangle>\<rangle>)\<^sup>\<sharp> \<circ>\<^sub>c zero)) \<circ>\<^sub>c \<langle>\<langle>a,b\<rangle>,id\<^sub>c one\<rangle>"
-    using assms by (typecheck_cfuncs, simp add: comp_associative2)
-    also have "... = (eval_func \<nat>\<^sub>c (\<nat>\<^sub>c\<times>\<^sub>c\<nat>\<^sub>c))\<circ>\<^sub>c 
-(id\<^sub>c (\<nat>\<^sub>c\<times>\<^sub>c\<nat>\<^sub>c) \<times>\<^sub>f ((mult2 \<circ>\<^sub>c (id\<^sub>c \<nat>\<^sub>c  \<times>\<^sub>f mult2) \<circ>\<^sub>c \<langle>(left_cart_proj \<nat>\<^sub>c \<nat>\<^sub>c) \<circ>\<^sub>c (left_cart_proj (\<nat>\<^sub>c\<times>\<^sub>c \<nat>\<^sub>c) \<nat>\<^sub>c),
-\<langle>(right_cart_proj \<nat>\<^sub>c \<nat>\<^sub>c) \<circ>\<^sub>c (left_cart_proj (\<nat>\<^sub>c\<times>\<^sub>c \<nat>\<^sub>c) \<nat>\<^sub>c), (right_cart_proj (\<nat>\<^sub>c\<times>\<^sub>c \<nat>\<^sub>c) \<nat>\<^sub>c)\<rangle>\<rangle>)\<^sup>\<sharp> )) \<circ>\<^sub>c (id\<^sub>c (\<nat>\<^sub>c\<times>\<^sub>c\<nat>\<^sub>c) \<times>\<^sub>f zero)  \<circ>\<^sub>c \<langle>\<langle>a,b\<rangle>,id\<^sub>c one\<rangle>"
-      using assms by (typecheck_cfuncs, smt comp_associative2 inv_transpose_func_def2 inv_transpose_of_composition transpose_func_def)
-    also have "... = (mult2 \<circ>\<^sub>c (id\<^sub>c \<nat>\<^sub>c  \<times>\<^sub>f mult2) \<circ>\<^sub>c \<langle>(left_cart_proj \<nat>\<^sub>c \<nat>\<^sub>c) \<circ>\<^sub>c (left_cart_proj (\<nat>\<^sub>c\<times>\<^sub>c \<nat>\<^sub>c) \<nat>\<^sub>c),
-\<langle>(right_cart_proj \<nat>\<^sub>c \<nat>\<^sub>c) \<circ>\<^sub>c (left_cart_proj (\<nat>\<^sub>c\<times>\<^sub>c \<nat>\<^sub>c) \<nat>\<^sub>c), (right_cart_proj (\<nat>\<^sub>c\<times>\<^sub>c \<nat>\<^sub>c) \<nat>\<^sub>c)\<rangle>\<rangle>)\<circ>\<^sub>c (id\<^sub>c (\<nat>\<^sub>c\<times>\<^sub>c\<nat>\<^sub>c) \<times>\<^sub>f zero)  \<circ>\<^sub>c \<langle>\<langle>a,b\<rangle>,id\<^sub>c one\<rangle>"
-       using assms by (typecheck_cfuncs, smt comp_associative2 transpose_func_def)
-    also have "... = mult2 \<circ>\<^sub>c (id\<^sub>c \<nat>\<^sub>c  \<times>\<^sub>f mult2) \<circ>\<^sub>c \<langle>(left_cart_proj \<nat>\<^sub>c \<nat>\<^sub>c) \<circ>\<^sub>c (left_cart_proj (\<nat>\<^sub>c\<times>\<^sub>c \<nat>\<^sub>c) \<nat>\<^sub>c),
-\<langle>(right_cart_proj \<nat>\<^sub>c \<nat>\<^sub>c) \<circ>\<^sub>c (left_cart_proj (\<nat>\<^sub>c\<times>\<^sub>c \<nat>\<^sub>c) \<nat>\<^sub>c), (right_cart_proj (\<nat>\<^sub>c\<times>\<^sub>c \<nat>\<^sub>c) \<nat>\<^sub>c)\<rangle>\<rangle>\<circ>\<^sub>c \<langle>id\<^sub>c (\<nat>\<^sub>c\<times>\<^sub>c\<nat>\<^sub>c) \<circ>\<^sub>c \<langle>a,b\<rangle>,zero \<circ>\<^sub>cid\<^sub>c one\<rangle>"
-    using assms by (typecheck_cfuncs, simp add: cfunc_cross_prod_comp_cfunc_prod comp_associative2)
+\<langle>(right_cart_proj \<nat>\<^sub>c \<nat>\<^sub>c) \<circ>\<^sub>c (left_cart_proj (\<nat>\<^sub>c\<times>\<^sub>c \<nat>\<^sub>c) \<nat>\<^sub>c), (right_cart_proj (\<nat>\<^sub>c\<times>\<^sub>c \<nat>\<^sub>c) \<nat>\<^sub>c)\<rangle>\<rangle>)\<^sup>\<sharp> \<circ>\<^sub>c zero))) \<circ>\<^sub>c x"
+              using comp_associative2 x_type y1_type by (typecheck_cfuncs, blast)
+           then show "(eval_func \<nat>\<^sub>c (\<nat>\<^sub>c \<times>\<^sub>c \<nat>\<^sub>c) \<circ>\<^sub>c id\<^sub>c (\<nat>\<^sub>c \<times>\<^sub>c \<nat>\<^sub>c) \<times>\<^sub>f (mult2 \<circ>\<^sub>c mult2 \<times>\<^sub>f id\<^sub>c \<nat>\<^sub>c)\<^sup>\<sharp> \<circ>\<^sub>c zero) \<circ>\<^sub>c x = (eval_func \<nat>\<^sub>c (\<nat>\<^sub>c \<times>\<^sub>c \<nat>\<^sub>c) \<circ>\<^sub>c id\<^sub>c (\<nat>\<^sub>c \<times>\<^sub>c \<nat>\<^sub>c) \<times>\<^sub>f (mult2 \<circ>\<^sub>c (id\<^sub>c \<nat>\<^sub>c \<times>\<^sub>f mult2) \<circ>\<^sub>c \<langle>left_cart_proj \<nat>\<^sub>c \<nat>\<^sub>c \<circ>\<^sub>c left_cart_proj (\<nat>\<^sub>c \<times>\<^sub>c \<nat>\<^sub>c) \<nat>\<^sub>c,\<langle>right_cart_proj \<nat>\<^sub>c \<nat>\<^sub>c \<circ>\<^sub>c left_cart_proj (\<nat>\<^sub>c \<times>\<^sub>c \<nat>\<^sub>c) \<nat>\<^sub>c,right_cart_proj (\<nat>\<^sub>c \<times>\<^sub>c \<nat>\<^sub>c) \<nat>\<^sub>c\<rangle>\<rangle>)\<^sup>\<sharp> \<circ>\<^sub>c zero) \<circ>\<^sub>c x"
+             by (simp add: calculation)
+         qed
+       qed
+     qed
+     show "(mult2 \<circ>\<^sub>c mult2 \<times>\<^sub>f id\<^sub>c \<nat>\<^sub>c)\<^sup>\<sharp> \<circ>\<^sub>c successor =
+    (add2 \<circ>\<^sub>c \<langle>mult2 \<circ>\<^sub>c left_cart_proj (\<nat>\<^sub>c \<times>\<^sub>c \<nat>\<^sub>c) (\<nat>\<^sub>c\<^bsup>(\<nat>\<^sub>c \<times>\<^sub>c \<nat>\<^sub>c)\<^esup>),eval_func \<nat>\<^sub>c (\<nat>\<^sub>c \<times>\<^sub>c \<nat>\<^sub>c)\<rangle>)\<^sup>\<sharp> \<circ>\<^sub>c (mult2 \<circ>\<^sub>c mult2 \<times>\<^sub>f id\<^sub>c \<nat>\<^sub>c)\<^sup>\<sharp>"
+     proof(rule same_evals_equal[where Z = "\<nat>\<^sub>c", where X = "\<nat>\<^sub>c", where A = "(\<nat>\<^sub>c\<times>\<^sub>c \<nat>\<^sub>c)"])
+       show "(mult2 \<circ>\<^sub>c mult2 \<times>\<^sub>f id\<^sub>c \<nat>\<^sub>c)\<^sup>\<sharp> \<circ>\<^sub>c successor : \<nat>\<^sub>c \<rightarrow>  \<nat>\<^sub>c\<^bsup>(\<nat>\<^sub>c\<times>\<^sub>c \<nat>\<^sub>c)\<^esup>"
+         using mmIdSharpS_type by blast
+       show type1: "(add2 \<circ>\<^sub>c \<langle>mult2 \<circ>\<^sub>c left_cart_proj (\<nat>\<^sub>c \<times>\<^sub>c \<nat>\<^sub>c) (\<nat>\<^sub>c\<^bsup>(\<nat>\<^sub>c \<times>\<^sub>c \<nat>\<^sub>c)\<^esup>),eval_func \<nat>\<^sub>c (\<nat>\<^sub>c \<times>\<^sub>c \<nat>\<^sub>c)\<rangle>)\<^sup>\<sharp> \<circ>\<^sub>c (mult2 \<circ>\<^sub>c mult2 \<times>\<^sub>f id\<^sub>c \<nat>\<^sub>c)\<^sup>\<sharp> : \<nat>\<^sub>c \<rightarrow> \<nat>\<^sub>c\<^bsup>(\<nat>\<^sub>c \<times>\<^sub>c \<nat>\<^sub>c)\<^esup>"
+         by (meson addMultSigma0EvalSharp_type comp_type multmultIdSharp_type)
+       show "eval_func \<nat>\<^sub>c (\<nat>\<^sub>c \<times>\<^sub>c \<nat>\<^sub>c) \<circ>\<^sub>c id\<^sub>c (\<nat>\<^sub>c \<times>\<^sub>c \<nat>\<^sub>c) \<times>\<^sub>f (mult2 \<circ>\<^sub>c mult2 \<times>\<^sub>f id\<^sub>c \<nat>\<^sub>c)\<^sup>\<sharp> \<circ>\<^sub>c successor = eval_func \<nat>\<^sub>c (\<nat>\<^sub>c \<times>\<^sub>c \<nat>\<^sub>c) \<circ>\<^sub>c id\<^sub>c (\<nat>\<^sub>c \<times>\<^sub>c \<nat>\<^sub>c) \<times>\<^sub>f (add2 \<circ>\<^sub>c \<langle>mult2 \<circ>\<^sub>c left_cart_proj (\<nat>\<^sub>c \<times>\<^sub>c \<nat>\<^sub>c) (\<nat>\<^sub>c\<^bsup>(\<nat>\<^sub>c \<times>\<^sub>c \<nat>\<^sub>c)\<^esup>),eval_func \<nat>\<^sub>c (\<nat>\<^sub>c \<times>\<^sub>c \<nat>\<^sub>c)\<rangle>)\<^sup>\<sharp> \<circ>\<^sub>c (mult2 \<circ>\<^sub>c mult2 \<times>\<^sub>f id\<^sub>c \<nat>\<^sub>c)\<^sup>\<sharp>"
+       proof(rule one_separator[where X ="(\<nat>\<^sub>c \<times>\<^sub>c \<nat>\<^sub>c)\<times>\<^sub>c \<nat>\<^sub>c", where Y = "\<nat>\<^sub>c"])
+         show "eval_func \<nat>\<^sub>c (\<nat>\<^sub>c \<times>\<^sub>c \<nat>\<^sub>c) \<circ>\<^sub>c
+    id\<^sub>c (\<nat>\<^sub>c \<times>\<^sub>c \<nat>\<^sub>c) \<times>\<^sub>f
+    (mult2 \<circ>\<^sub>c mult2 \<times>\<^sub>f id\<^sub>c \<nat>\<^sub>c)\<^sup>\<sharp> \<circ>\<^sub>c successor : (\<nat>\<^sub>c \<times>\<^sub>c \<nat>\<^sub>c)\<times>\<^sub>c \<nat>\<^sub>c \<rightarrow> \<nat>\<^sub>c"
+           using flat_type inv_transpose_func_def2 mmIdSharpS_type by auto
+         show "eval_func \<nat>\<^sub>c (\<nat>\<^sub>c \<times>\<^sub>c \<nat>\<^sub>c) \<circ>\<^sub>c id\<^sub>c (\<nat>\<^sub>c \<times>\<^sub>c \<nat>\<^sub>c) \<times>\<^sub>f (add2 \<circ>\<^sub>c \<langle>mult2 \<circ>\<^sub>c left_cart_proj (\<nat>\<^sub>c \<times>\<^sub>c \<nat>\<^sub>c) (\<nat>\<^sub>c\<^bsup>(\<nat>\<^sub>c \<times>\<^sub>c \<nat>\<^sub>c)\<^esup>),eval_func \<nat>\<^sub>c (\<nat>\<^sub>c \<times>\<^sub>c \<nat>\<^sub>c)\<rangle>)\<^sup>\<sharp> \<circ>\<^sub>c (mult2 \<circ>\<^sub>c mult2 \<times>\<^sub>f id\<^sub>c \<nat>\<^sub>c)\<^sup>\<sharp> : (\<nat>\<^sub>c \<times>\<^sub>c \<nat>\<^sub>c) \<times>\<^sub>c \<nat>\<^sub>c \<rightarrow> \<nat>\<^sub>c"
+           using flat_type inv_transpose_func_def2 type1 by auto
+         show "\<And>x. x \<in>\<^sub>c (\<nat>\<^sub>c \<times>\<^sub>c \<nat>\<^sub>c) \<times>\<^sub>c \<nat>\<^sub>c \<Longrightarrow>
+         (eval_func \<nat>\<^sub>c (\<nat>\<^sub>c \<times>\<^sub>c \<nat>\<^sub>c) \<circ>\<^sub>c id\<^sub>c (\<nat>\<^sub>c \<times>\<^sub>c \<nat>\<^sub>c) \<times>\<^sub>f
+          (mult2 \<circ>\<^sub>c mult2 \<times>\<^sub>f id\<^sub>c \<nat>\<^sub>c)\<^sup>\<sharp> \<circ>\<^sub>c successor) \<circ>\<^sub>c x =
+ (eval_func \<nat>\<^sub>c (\<nat>\<^sub>c \<times>\<^sub>c \<nat>\<^sub>c) \<circ>\<^sub>c id\<^sub>c (\<nat>\<^sub>c \<times>\<^sub>c \<nat>\<^sub>c) \<times>\<^sub>f (add2 \<circ>\<^sub>c \<langle>mult2 \<circ>\<^sub>c left_cart_proj (\<nat>\<^sub>c \<times>\<^sub>c \<nat>\<^sub>c) (\<nat>\<^sub>c\<^bsup>(\<nat>\<^sub>c \<times>\<^sub>c \<nat>\<^sub>c)\<^esup>),eval_func \<nat>\<^sub>c (\<nat>\<^sub>c \<times>\<^sub>c \<nat>\<^sub>c)\<rangle>)\<^sup>\<sharp> \<circ>\<^sub>c (mult2 \<circ>\<^sub>c mult2 \<times>\<^sub>f id\<^sub>c \<nat>\<^sub>c)\<^sup>\<sharp>) \<circ>\<^sub>c x"
+         proof - 
+           fix x 
+           assume x_type: "x \<in>\<^sub>c (\<nat>\<^sub>c \<times>\<^sub>c \<nat>\<^sub>c) \<times>\<^sub>c \<nat>\<^sub>c"
+           obtain y r where x_def: "y \<in>\<^sub>c (\<nat>\<^sub>c \<times>\<^sub>c \<nat>\<^sub>c) \<and> r \<in>\<^sub>c \<nat>\<^sub>c \<and> x = \<langle>y,r\<rangle>"
+             using cart_prod_decomp x_type by blast
+           obtain p q where y_def: "p  \<in>\<^sub>c \<nat>\<^sub>c \<and> q \<in>\<^sub>c \<nat>\<^sub>c \<and> y = \<langle>p,q\<rangle>"
+             using cart_prod_decomp x_def by blast
+           have pq_type: "\<langle>p,q\<rangle> \<in>\<^sub>c (\<nat>\<^sub>c \<times>\<^sub>c \<nat>\<^sub>c)"
+             using x_def y_def by force
+           have y_type: "y \<in>\<^sub>c (\<nat>\<^sub>c \<times>\<^sub>c \<nat>\<^sub>c)"
+             by (simp add: x_def)
+           have x_def2: "x = \<langle>\<langle>p,q\<rangle>,r\<rangle>"
+             using x_def y_def by blast
+           have ysr_type: "\<langle>y,successor \<circ>\<^sub>c  r\<rangle> \<in>\<^sub>c (\<nat>\<^sub>c \<times>\<^sub>c \<nat>\<^sub>c) \<times>\<^sub>c \<nat>\<^sub>c"
+             by (simp add: cfunc_prod_type succ_n_type x_def)
 
-    also have "... = mult2 \<circ>\<^sub>c (id\<^sub>c \<nat>\<^sub>c  \<times>\<^sub>f mult2) \<circ>\<^sub>c \<langle>(left_cart_proj \<nat>\<^sub>c \<nat>\<^sub>c) \<circ>\<^sub>c (left_cart_proj (\<nat>\<^sub>c\<times>\<^sub>c \<nat>\<^sub>c) \<nat>\<^sub>c),
-\<langle>(right_cart_proj \<nat>\<^sub>c \<nat>\<^sub>c) \<circ>\<^sub>c (left_cart_proj (\<nat>\<^sub>c\<times>\<^sub>c \<nat>\<^sub>c) \<nat>\<^sub>c), (right_cart_proj (\<nat>\<^sub>c\<times>\<^sub>c \<nat>\<^sub>c) \<nat>\<^sub>c)\<rangle>\<rangle>\<circ>\<^sub>c \<langle>\<langle>a,b\<rangle>,zero\<rangle>"
-      using ab_type id_left_unit2 id_right_unit2 zero_type by auto
-    also have "... = mult2 \<circ>\<^sub>c (id\<^sub>c \<nat>\<^sub>c  \<times>\<^sub>f mult2) \<circ>\<^sub>c \<langle>(left_cart_proj \<nat>\<^sub>c \<nat>\<^sub>c) \<circ>\<^sub>c (left_cart_proj (\<nat>\<^sub>c\<times>\<^sub>c \<nat>\<^sub>c) \<nat>\<^sub>c) \<circ>\<^sub>c \<langle>\<langle>a,b\<rangle>,zero\<rangle>,
-\<langle>(right_cart_proj \<nat>\<^sub>c \<nat>\<^sub>c) \<circ>\<^sub>c (left_cart_proj (\<nat>\<^sub>c\<times>\<^sub>c \<nat>\<^sub>c) \<nat>\<^sub>c), (right_cart_proj (\<nat>\<^sub>c\<times>\<^sub>c \<nat>\<^sub>c) \<nat>\<^sub>c)\<rangle> \<circ>\<^sub>c \<langle>\<langle>a,b\<rangle>,zero\<rangle>  \<rangle>"
-     using assms by (typecheck_cfuncs, simp add: cfunc_prod_comp comp_associative2)
-   also have "... = mult2 \<circ>\<^sub>c (id\<^sub>c \<nat>\<^sub>c  \<times>\<^sub>f mult2) \<circ>\<^sub>c \<langle>(left_cart_proj \<nat>\<^sub>c \<nat>\<^sub>c) \<circ>\<^sub>c (left_cart_proj (\<nat>\<^sub>c\<times>\<^sub>c \<nat>\<^sub>c) \<nat>\<^sub>c) \<circ>\<^sub>c \<langle>\<langle>a,b\<rangle>,zero\<rangle>,
-\<langle>(right_cart_proj \<nat>\<^sub>c \<nat>\<^sub>c) \<circ>\<^sub>c (left_cart_proj (\<nat>\<^sub>c\<times>\<^sub>c \<nat>\<^sub>c) \<nat>\<^sub>c) \<circ>\<^sub>c \<langle>\<langle>a,b\<rangle>,zero\<rangle>  , (right_cart_proj (\<nat>\<^sub>c\<times>\<^sub>c \<nat>\<^sub>c) \<nat>\<^sub>c) \<circ>\<^sub>c \<langle>\<langle>a,b\<rangle>,zero\<rangle>  \<rangle>  \<rangle>"
-         using assms by (typecheck_cfuncs, simp add: cfunc_prod_comp comp_associative2)
-   also have "... = mult2 \<circ>\<^sub>c (id\<^sub>c \<nat>\<^sub>c  \<times>\<^sub>f mult2) \<circ>\<^sub>c \<langle>(left_cart_proj \<nat>\<^sub>c \<nat>\<^sub>c) \<circ>\<^sub>c  \<langle>a,b\<rangle>,
-\<langle>(right_cart_proj \<nat>\<^sub>c \<nat>\<^sub>c) \<circ>\<^sub>c  \<langle>a,b\<rangle>  ,zero  \<rangle>  \<rangle>"
-     using ab_type left_cart_proj_cfunc_prod right_cart_proj_cfunc_prod zero_type by auto
-   also have "... = mult2 \<circ>\<^sub>c (id\<^sub>c \<nat>\<^sub>c  \<times>\<^sub>f mult2) \<circ>\<^sub>c \<langle>a , \<langle>b,zero\<rangle>  \<rangle>"
-     using assms(1) assms(2) left_cart_proj_cfunc_prod right_cart_proj_cfunc_prod by auto
-   also have "... = mult2 \<circ>\<^sub>c  \<langle>id\<^sub>c \<nat>\<^sub>c \<circ>\<^sub>c a ,mult2 \<circ>\<^sub>c \<langle>b,zero\<rangle>  \<rangle>"
-     using assms(1) b0_type id_type mult2_type cfunc_cross_prod_comp_cfunc_prod by fastforce
-   also have "... = zero"
-     using assms(1) assms(2) id_left_unit2 mult_def mult_respects_zero_right by auto
-        then show ?thesis using calculation by auto
-qed
+           have "(eval_func \<nat>\<^sub>c (\<nat>\<^sub>c \<times>\<^sub>c \<nat>\<^sub>c) \<circ>\<^sub>c id\<^sub>c (\<nat>\<^sub>c \<times>\<^sub>c \<nat>\<^sub>c) \<times>\<^sub>f
+          (mult2 \<circ>\<^sub>c mult2 \<times>\<^sub>f id\<^sub>c \<nat>\<^sub>c)\<^sup>\<sharp> \<circ>\<^sub>c successor) \<circ>\<^sub>c x = 
+            ((eval_func \<nat>\<^sub>c (\<nat>\<^sub>c \<times>\<^sub>c \<nat>\<^sub>c) \<circ>\<^sub>c id\<^sub>c (\<nat>\<^sub>c \<times>\<^sub>c \<nat>\<^sub>c) \<times>\<^sub>f
+          (mult2 \<circ>\<^sub>c mult2 \<times>\<^sub>f id\<^sub>c \<nat>\<^sub>c)\<^sup>\<sharp>) \<circ>\<^sub>c (id\<^sub>c (\<nat>\<^sub>c \<times>\<^sub>c \<nat>\<^sub>c) \<times>\<^sub>f successor)) \<circ>\<^sub>c x"
+             by (typecheck_cfuncs, metis inv_transpose_func_def2 inv_transpose_of_composition)
+           also have "... = ((eval_func \<nat>\<^sub>c (\<nat>\<^sub>c \<times>\<^sub>c \<nat>\<^sub>c) \<circ>\<^sub>c id\<^sub>c (\<nat>\<^sub>c \<times>\<^sub>c \<nat>\<^sub>c) \<times>\<^sub>f
+          (mult2 \<circ>\<^sub>c mult2 \<times>\<^sub>f id\<^sub>c \<nat>\<^sub>c)\<^sup>\<sharp>) \<circ>\<^sub>c (id\<^sub>c (\<nat>\<^sub>c \<times>\<^sub>c \<nat>\<^sub>c) \<times>\<^sub>f successor) \<circ>\<^sub>c x)"
+             using comp_associative2 x_type by (typecheck_cfuncs, auto)
+           also have "... = (mult2 \<circ>\<^sub>c mult2 \<times>\<^sub>f id\<^sub>c \<nat>\<^sub>c) \<circ>\<^sub>c ((id\<^sub>c (\<nat>\<^sub>c \<times>\<^sub>c \<nat>\<^sub>c) \<times>\<^sub>f successor) \<circ>\<^sub>c x)"
+             by (typecheck_cfuncs, simp add: transpose_func_def)
+           also have "... = (mult2 \<circ>\<^sub>c mult2 \<times>\<^sub>f id\<^sub>c \<nat>\<^sub>c) \<circ>\<^sub>c ((id\<^sub>c (\<nat>\<^sub>c \<times>\<^sub>c \<nat>\<^sub>c) \<times>\<^sub>f successor) \<circ>\<^sub>c \<langle>y,r\<rangle>)"
+             using x_def by blast
+           also have "... = (mult2 \<circ>\<^sub>c mult2 \<times>\<^sub>f id\<^sub>c \<nat>\<^sub>c) \<circ>\<^sub>c  \<langle>id\<^sub>c (\<nat>\<^sub>c \<times>\<^sub>c \<nat>\<^sub>c)\<circ>\<^sub>c y,successor \<circ>\<^sub>c  r\<rangle>"
+             using cfunc_cross_prod_comp_cfunc_prod x_def by (typecheck_cfuncs, auto)
+           also have "... = (mult2 \<circ>\<^sub>c (mult2 \<times>\<^sub>f id\<^sub>c \<nat>\<^sub>c)) \<circ>\<^sub>c  \<langle>y,successor \<circ>\<^sub>c  r\<rangle>"
+             using id_left_unit2 x_def by auto
+           also have "... = mult2 \<circ>\<^sub>c (mult2 \<times>\<^sub>f id\<^sub>c \<nat>\<^sub>c) \<circ>\<^sub>c  \<langle>y,successor \<circ>\<^sub>c  r\<rangle>"
+             using comp_associative2 ysr_type by (typecheck_cfuncs, auto)
+           also have "... = mult2 \<circ>\<^sub>c \<langle>mult2 \<circ>\<^sub>c y,id\<^sub>c \<nat>\<^sub>c \<circ>\<^sub>c (successor \<circ>\<^sub>c  r)\<rangle>"
+             by (typecheck_cfuncs, smt cfunc_cross_prod_comp_cfunc_prod x_def)
+           also have "... = mult2 \<circ>\<^sub>c \<langle>p \<cdot>\<^sub>\<nat> q, successor \<circ>\<^sub>c  r\<rangle>"
+             using cfunc_type_def comp_associative id_domain id_left_unit2 mult_def successor_type x_def y_def by auto
+           also have "... = (p \<cdot>\<^sub>\<nat> q) \<cdot>\<^sub>\<nat> (successor \<circ>\<^sub>c  r)"
+             by (simp add: mult_def)
+           also have "... = (p \<cdot>\<^sub>\<nat> q) +\<^sub>\<nat> ((p \<cdot>\<^sub>\<nat> q)\<cdot>\<^sub>\<nat> r)"
+             by (simp add: mult_closure mult_respects_succ_right x_def y_def)
+           also have "... = add2 \<circ>\<^sub>c\<langle>p \<cdot>\<^sub>\<nat> q,(p \<cdot>\<^sub>\<nat> q)\<cdot>\<^sub>\<nat> r\<rangle>"
+             by (simp add: add_def)
+           also have "... = add2 \<circ>\<^sub>c\<langle>mult2\<circ>\<^sub>c \<langle>p,q\<rangle>,mult2\<circ>\<^sub>c \<langle>(p \<cdot>\<^sub>\<nat> q),r\<rangle>\<rangle>"
+             using mult_def by fastforce
+           also have "... = add2 \<circ>\<^sub>c\<langle>mult2\<circ>\<^sub>c \<langle>p,q\<rangle>,mult2\<circ>\<^sub>c \<langle>mult2\<circ>\<^sub>c \<langle>p,q\<rangle>, id\<^sub>c \<nat>\<^sub>c \<circ>\<^sub>c r\<rangle>\<rangle>"
+             using id_left_unit2 mult_def x_def by force
+           also have "... =  add2 \<circ>\<^sub>c\<langle>mult2 \<circ>\<^sub>c  \<langle>p,q\<rangle> ,(mult2 \<circ>\<^sub>c (mult2 \<times>\<^sub>f id\<^sub>c \<nat>\<^sub>c)) \<circ>\<^sub>c\<langle>\<langle>p,q\<rangle>,r\<rangle>   \<rangle>"
+             by (typecheck_cfuncs, smt cfunc_cross_prod_comp_cfunc_prod comp_associative2 x_def x_type y_def)
+          also have "... = add2 \<circ>\<^sub>c
+\<langle>mult2 \<circ>\<^sub>c left_cart_proj (\<nat>\<^sub>c\<times>\<^sub>c\<nat>\<^sub>c) \<nat>\<^sub>c \<circ>\<^sub>c\<langle>\<langle>p,q\<rangle>,r\<rangle> ,
+eval_func \<nat>\<^sub>c (\<nat>\<^sub>c\<times>\<^sub>c\<nat>\<^sub>c)
+\<circ>\<^sub>c (id\<^sub>c (\<nat>\<^sub>c\<times>\<^sub>c\<nat>\<^sub>c) \<times>\<^sub>f ((mult2 \<circ>\<^sub>c (mult2 \<times>\<^sub>f id\<^sub>c \<nat>\<^sub>c))\<^sup>\<sharp>))\<circ>\<^sub>c\<langle>\<langle>p,q\<rangle>,r\<rangle>   \<rangle>"
+            by (typecheck_cfuncs, smt comp_associative2 left_cart_proj_cfunc_prod transpose_func_def x_def y_def)
+          
+          also have "... = add2 \<circ>\<^sub>c \<langle>mult2 \<circ>\<^sub>c left_cart_proj (\<nat>\<^sub>c\<times>\<^sub>c\<nat>\<^sub>c) \<nat>\<^sub>c , eval_func \<nat>\<^sub>c (\<nat>\<^sub>c\<times>\<^sub>c\<nat>\<^sub>c) \<circ>\<^sub>c (id\<^sub>c (\<nat>\<^sub>c\<times>\<^sub>c\<nat>\<^sub>c) \<times>\<^sub>f ((mult2 \<circ>\<^sub>c (mult2 \<times>\<^sub>f id\<^sub>c \<nat>\<^sub>c))\<^sup>\<sharp>))\<rangle>  \<circ>\<^sub>c\<langle>\<langle>p,q\<rangle>,r\<rangle>"
+            using cfunc_prod_comp comp_associative2 x_def2 x_type by (typecheck_cfuncs, auto)
+          also have "... = (add2 \<circ>\<^sub>c \<langle>mult2 \<circ>\<^sub>c (id\<^sub>c (\<nat>\<^sub>c\<times>\<^sub>c\<nat>\<^sub>c) \<circ>\<^sub>c left_cart_proj (\<nat>\<^sub>c\<times>\<^sub>c\<nat>\<^sub>c) \<nat>\<^sub>c) , eval_func \<nat>\<^sub>c (\<nat>\<^sub>c\<times>\<^sub>c\<nat>\<^sub>c) \<circ>\<^sub>c (id\<^sub>c (\<nat>\<^sub>c\<times>\<^sub>c\<nat>\<^sub>c) \<times>\<^sub>f ((mult2 \<circ>\<^sub>c (mult2 \<times>\<^sub>f id\<^sub>c \<nat>\<^sub>c))\<^sup>\<sharp>))\<rangle>  ) \<circ>\<^sub>c\<langle>\<langle>p,q\<rangle>,r\<rangle>"
+            using comp_associative2 id_left_unit2 x_def2 x_type by (typecheck_cfuncs, auto)
+          also have "... = (add2 \<circ>\<^sub>c \<langle>mult2 \<circ>\<^sub>c (left_cart_proj (\<nat>\<^sub>c\<times>\<^sub>c\<nat>\<^sub>c) (\<nat>\<^sub>c\<^bsup>(\<nat>\<^sub>c\<times>\<^sub>c\<nat>\<^sub>c)\<^esup>)) \<circ>\<^sub>c (id\<^sub>c (\<nat>\<^sub>c\<times>\<^sub>c\<nat>\<^sub>c) \<times>\<^sub>f ((mult2 \<circ>\<^sub>c (mult2 \<times>\<^sub>f id\<^sub>c \<nat>\<^sub>c))\<^sup>\<sharp>)), eval_func \<nat>\<^sub>c (\<nat>\<^sub>c\<times>\<^sub>c\<nat>\<^sub>c) \<circ>\<^sub>c (id\<^sub>c (\<nat>\<^sub>c\<times>\<^sub>c\<nat>\<^sub>c) \<times>\<^sub>f ((mult2 \<circ>\<^sub>c (mult2 \<times>\<^sub>f id\<^sub>c \<nat>\<^sub>c))\<^sup>\<sharp>))\<rangle>  ) \<circ>\<^sub>c\<langle>\<langle>p,q\<rangle>,r\<rangle>"
+            by (typecheck_cfuncs, simp add: left_cart_proj_cfunc_cross_prod)
+          also have "... = ((add2 \<circ>\<^sub>c \<langle>mult2 \<circ>\<^sub>c (left_cart_proj (\<nat>\<^sub>c\<times>\<^sub>c\<nat>\<^sub>c) (\<nat>\<^sub>c\<^bsup>(\<nat>\<^sub>c\<times>\<^sub>c\<nat>\<^sub>c)\<^esup>)), eval_func \<nat>\<^sub>c (\<nat>\<^sub>c\<times>\<^sub>c\<nat>\<^sub>c)\<rangle>)  \<circ>\<^sub>c (id\<^sub>c (\<nat>\<^sub>c\<times>\<^sub>c\<nat>\<^sub>c) \<times>\<^sub>f ((mult2 \<circ>\<^sub>c (mult2 \<times>\<^sub>f id\<^sub>c \<nat>\<^sub>c))\<^sup>\<sharp>))) \<circ>\<^sub>c\<langle>\<langle>p,q\<rangle>,r\<rangle>"
+            by (typecheck_cfuncs, smt cfunc_prod_comp cfunc_type_def comp_associative)
+          also have "... = (add2 \<circ>\<^sub>c \<langle>mult2 \<circ>\<^sub>c (left_cart_proj (\<nat>\<^sub>c\<times>\<^sub>c\<nat>\<^sub>c) (\<nat>\<^sub>c\<^bsup>(\<nat>\<^sub>c\<times>\<^sub>c\<nat>\<^sub>c)\<^esup>)),eval_func \<nat>\<^sub>c (\<nat>\<^sub>c\<times>\<^sub>c\<nat>\<^sub>c)\<rangle>) \<circ>\<^sub>c (id\<^sub>c (\<nat>\<^sub>c\<times>\<^sub>c\<nat>\<^sub>c) \<times>\<^sub>f ((mult2 \<circ>\<^sub>c (mult2 \<times>\<^sub>f id\<^sub>c \<nat>\<^sub>c))\<^sup>\<sharp>))\<circ>\<^sub>c \<langle>\<langle>p,q\<rangle>,r\<rangle>"  
+            using comp_associative2 x_def2 x_type by (typecheck_cfuncs, auto)
+          also have "... = (eval_func \<nat>\<^sub>c (\<nat>\<^sub>c\<times>\<^sub>c\<nat>\<^sub>c))\<circ>\<^sub>c (id\<^sub>c (\<nat>\<^sub>c\<times>\<^sub>c\<nat>\<^sub>c) \<times>\<^sub>f ((add2 \<circ>\<^sub>c \<langle>mult2 \<circ>\<^sub>c (left_cart_proj (\<nat>\<^sub>c\<times>\<^sub>c\<nat>\<^sub>c) (\<nat>\<^sub>c\<^bsup>(\<nat>\<^sub>c\<times>\<^sub>c\<nat>\<^sub>c)\<^esup>)),eval_func \<nat>\<^sub>c (\<nat>\<^sub>c\<times>\<^sub>c\<nat>\<^sub>c)\<rangle>)\<^sup>\<sharp>)) \<circ>\<^sub>c (id\<^sub>c (\<nat>\<^sub>c\<times>\<^sub>c\<nat>\<^sub>c) \<times>\<^sub>f ((mult2 \<circ>\<^sub>c (mult2 \<times>\<^sub>f id\<^sub>c \<nat>\<^sub>c))\<^sup>\<sharp>))\<circ>\<^sub>c \<langle>\<langle>p,q\<rangle>,r\<rangle>"
+              by (typecheck_cfuncs , smt comp_associative2 transpose_func_def x_def2 x_type)
+          also have "... =  (eval_func \<nat>\<^sub>c (\<nat>\<^sub>c\<times>\<^sub>c\<nat>\<^sub>c))\<circ>\<^sub>c (id\<^sub>c (\<nat>\<^sub>c\<times>\<^sub>c\<nat>\<^sub>c) \<times>\<^sub>f ((add2 \<circ>\<^sub>c \<langle>mult2 \<circ>\<^sub>c (left_cart_proj (\<nat>\<^sub>c\<times>\<^sub>c\<nat>\<^sub>c) (\<nat>\<^sub>c\<^bsup>(\<nat>\<^sub>c\<times>\<^sub>c\<nat>\<^sub>c)\<^esup>)),eval_func \<nat>\<^sub>c (\<nat>\<^sub>c\<times>\<^sub>c\<nat>\<^sub>c)\<rangle>)\<^sup>\<sharp>)\<circ>\<^sub>c ((mult2 \<circ>\<^sub>c (mult2 \<times>\<^sub>f id\<^sub>c \<nat>\<^sub>c))\<^sup>\<sharp>))  \<circ>\<^sub>c \<langle>\<langle>p,q\<rangle>,r\<rangle>"
+            by (typecheck_cfuncs, smt comp_associative2 inv_transpose_func_def2 inv_transpose_of_composition transpose_func_def x_def2 x_type)
+          also have "... = ((eval_func \<nat>\<^sub>c (\<nat>\<^sub>c\<times>\<^sub>c\<nat>\<^sub>c))\<circ>\<^sub>c  (id\<^sub>c (\<nat>\<^sub>c\<times>\<^sub>c\<nat>\<^sub>c) \<times>\<^sub>f ((add2 \<circ>\<^sub>c \<langle>mult2 \<circ>\<^sub>c (left_cart_proj (\<nat>\<^sub>c\<times>\<^sub>c\<nat>\<^sub>c) (\<nat>\<^sub>c\<^bsup>(\<nat>\<^sub>c\<times>\<^sub>c\<nat>\<^sub>c)\<^esup>)),eval_func \<nat>\<^sub>c (\<nat>\<^sub>c\<times>\<^sub>c\<nat>\<^sub>c)\<rangle>)\<^sup>\<sharp>)\<circ>\<^sub>c ((mult2 \<circ>\<^sub>c (mult2 \<times>\<^sub>f id\<^sub>c \<nat>\<^sub>c))\<^sup>\<sharp>) ))  \<circ>\<^sub>c x "
+            using comp_associative2 x_def2 x_type by (typecheck_cfuncs, blast)
+          then show "(eval_func \<nat>\<^sub>c (\<nat>\<^sub>c \<times>\<^sub>c \<nat>\<^sub>c) \<circ>\<^sub>c id\<^sub>c (\<nat>\<^sub>c \<times>\<^sub>c \<nat>\<^sub>c) \<times>\<^sub>f (mult2 \<circ>\<^sub>c mult2 \<times>\<^sub>f id\<^sub>c \<nat>\<^sub>c)\<^sup>\<sharp> \<circ>\<^sub>c successor) \<circ>\<^sub>c x = (eval_func \<nat>\<^sub>c (\<nat>\<^sub>c \<times>\<^sub>c \<nat>\<^sub>c) \<circ>\<^sub>c id\<^sub>c (\<nat>\<^sub>c \<times>\<^sub>c \<nat>\<^sub>c) \<times>\<^sub>f (add2 \<circ>\<^sub>c \<langle>mult2 \<circ>\<^sub>c left_cart_proj (\<nat>\<^sub>c \<times>\<^sub>c \<nat>\<^sub>c) (\<nat>\<^sub>c\<^bsup>(\<nat>\<^sub>c \<times>\<^sub>c \<nat>\<^sub>c)\<^esup>),eval_func \<nat>\<^sub>c (\<nat>\<^sub>c \<times>\<^sub>c \<nat>\<^sub>c)\<rangle>)\<^sup>\<sharp> \<circ>\<^sub>c (mult2 \<circ>\<^sub>c mult2 \<times>\<^sub>f id\<^sub>c \<nat>\<^sub>c)\<^sup>\<sharp>) \<circ>\<^sub>c x"
+            by (simp add: calculation)
+        qed
+      qed
+    qed
+    show "(mult2 \<circ>\<^sub>c (id\<^sub>c \<nat>\<^sub>c \<times>\<^sub>f mult2) \<circ>\<^sub>c \<langle>left_cart_proj \<nat>\<^sub>c \<nat>\<^sub>c \<circ>\<^sub>c left_cart_proj (\<nat>\<^sub>c \<times>\<^sub>c \<nat>\<^sub>c) \<nat>\<^sub>c,\<langle>right_cart_proj \<nat>\<^sub>c \<nat>\<^sub>c \<circ>\<^sub>c left_cart_proj (\<nat>\<^sub>c \<times>\<^sub>c \<nat>\<^sub>c) \<nat>\<^sub>c,right_cart_proj (\<nat>\<^sub>c \<times>\<^sub>c \<nat>\<^sub>c) \<nat>\<^sub>c\<rangle>\<rangle>)\<^sup>\<sharp> \<circ>\<^sub>c successor = (add2 \<circ>\<^sub>c \<langle>mult2 \<circ>\<^sub>c left_cart_proj (\<nat>\<^sub>c \<times>\<^sub>c \<nat>\<^sub>c) (\<nat>\<^sub>c\<^bsup>(\<nat>\<^sub>c \<times>\<^sub>c \<nat>\<^sub>c)\<^esup>),eval_func \<nat>\<^sub>c (\<nat>\<^sub>c \<times>\<^sub>c \<nat>\<^sub>c)\<rangle>)\<^sup>\<sharp> \<circ>\<^sub>c (mult2 \<circ>\<^sub>c (id\<^sub>c \<nat>\<^sub>c \<times>\<^sub>f mult2) \<circ>\<^sub>c \<langle>left_cart_proj \<nat>\<^sub>c \<nat>\<^sub>c \<circ>\<^sub>c left_cart_proj (\<nat>\<^sub>c \<times>\<^sub>c \<nat>\<^sub>c) \<nat>\<^sub>c,\<langle>right_cart_proj \<nat>\<^sub>c \<nat>\<^sub>c \<circ>\<^sub>c left_cart_proj (\<nat>\<^sub>c \<times>\<^sub>c \<nat>\<^sub>c) \<nat>\<^sub>c,right_cart_proj (\<nat>\<^sub>c \<times>\<^sub>c \<nat>\<^sub>c) \<nat>\<^sub>c\<rangle>\<rangle>)\<^sup>\<sharp>"
+    proof(rule same_evals_equal[where Z = "\<nat>\<^sub>c", where X = "\<nat>\<^sub>c", where A = "(\<nat>\<^sub>c\<times>\<^sub>c \<nat>\<^sub>c)"])
+      show "(mult2 \<circ>\<^sub>c (id\<^sub>c \<nat>\<^sub>c \<times>\<^sub>f mult2) \<circ>\<^sub>c \<langle>left_cart_proj \<nat>\<^sub>c \<nat>\<^sub>c \<circ>\<^sub>c left_cart_proj (\<nat>\<^sub>c \<times>\<^sub>c \<nat>\<^sub>c) \<nat>\<^sub>c,\<langle>right_cart_proj \<nat>\<^sub>c \<nat>\<^sub>c \<circ>\<^sub>c left_cart_proj (\<nat>\<^sub>c \<times>\<^sub>c \<nat>\<^sub>c) \<nat>\<^sub>c,right_cart_proj (\<nat>\<^sub>c \<times>\<^sub>c \<nat>\<^sub>c) \<nat>\<^sub>c\<rangle>\<rangle>)\<^sup>\<sharp> \<circ>\<^sub>c successor : \<nat>\<^sub>c \<rightarrow> \<nat>\<^sub>c\<^bsup>(\<nat>\<^sub>c \<times>\<^sub>c \<nat>\<^sub>c)\<^esup>"
+        by (simp add: multIdxMultp0p0p1p0p0_SharpSucc_type)
+      show type2: "(add2 \<circ>\<^sub>c \<langle>mult2 \<circ>\<^sub>c left_cart_proj (\<nat>\<^sub>c \<times>\<^sub>c \<nat>\<^sub>c) (\<nat>\<^sub>c\<^bsup>(\<nat>\<^sub>c \<times>\<^sub>c \<nat>\<^sub>c)\<^esup>),eval_func \<nat>\<^sub>c (\<nat>\<^sub>c \<times>\<^sub>c \<nat>\<^sub>c)\<rangle>)\<^sup>\<sharp> \<circ>\<^sub>c (mult2 \<circ>\<^sub>c (id\<^sub>c \<nat>\<^sub>c \<times>\<^sub>f mult2) \<circ>\<^sub>c \<langle>left_cart_proj \<nat>\<^sub>c \<nat>\<^sub>c \<circ>\<^sub>c left_cart_proj (\<nat>\<^sub>c \<times>\<^sub>c \<nat>\<^sub>c) \<nat>\<^sub>c,\<langle>right_cart_proj \<nat>\<^sub>c \<nat>\<^sub>c \<circ>\<^sub>c left_cart_proj (\<nat>\<^sub>c \<times>\<^sub>c \<nat>\<^sub>c) \<nat>\<^sub>c,right_cart_proj (\<nat>\<^sub>c \<times>\<^sub>c \<nat>\<^sub>c) \<nat>\<^sub>c\<rangle>\<rangle>)\<^sup>\<sharp> : \<nat>\<^sub>c \<rightarrow> \<nat>\<^sub>c\<^bsup>(\<nat>\<^sub>c \<times>\<^sub>c \<nat>\<^sub>c)\<^esup>"
+        using addMultSigma0EvalSharp_type comp_type multIdxMultp0p0p1p0p1_Sharp_type by blast
+      show "eval_func \<nat>\<^sub>c (\<nat>\<^sub>c \<times>\<^sub>c \<nat>\<^sub>c) \<circ>\<^sub>c id\<^sub>c (\<nat>\<^sub>c \<times>\<^sub>c \<nat>\<^sub>c) \<times>\<^sub>f (mult2 \<circ>\<^sub>c (id\<^sub>c \<nat>\<^sub>c \<times>\<^sub>f mult2) \<circ>\<^sub>c \<langle>left_cart_proj \<nat>\<^sub>c \<nat>\<^sub>c \<circ>\<^sub>c left_cart_proj (\<nat>\<^sub>c \<times>\<^sub>c \<nat>\<^sub>c) \<nat>\<^sub>c,\<langle>right_cart_proj \<nat>\<^sub>c \<nat>\<^sub>c \<circ>\<^sub>c left_cart_proj (\<nat>\<^sub>c \<times>\<^sub>c \<nat>\<^sub>c) \<nat>\<^sub>c,right_cart_proj (\<nat>\<^sub>c \<times>\<^sub>c \<nat>\<^sub>c) \<nat>\<^sub>c\<rangle>\<rangle>)\<^sup>\<sharp> \<circ>\<^sub>c successor = eval_func \<nat>\<^sub>c (\<nat>\<^sub>c \<times>\<^sub>c \<nat>\<^sub>c) \<circ>\<^sub>c id\<^sub>c (\<nat>\<^sub>c \<times>\<^sub>c \<nat>\<^sub>c) \<times>\<^sub>f (add2 \<circ>\<^sub>c \<langle>mult2 \<circ>\<^sub>c left_cart_proj (\<nat>\<^sub>c \<times>\<^sub>c \<nat>\<^sub>c) (\<nat>\<^sub>c\<^bsup>(\<nat>\<^sub>c \<times>\<^sub>c \<nat>\<^sub>c)\<^esup>),eval_func \<nat>\<^sub>c (\<nat>\<^sub>c \<times>\<^sub>c \<nat>\<^sub>c)\<rangle>)\<^sup>\<sharp> \<circ>\<^sub>c (mult2 \<circ>\<^sub>c (id\<^sub>c \<nat>\<^sub>c \<times>\<^sub>f mult2) \<circ>\<^sub>c \<langle>left_cart_proj \<nat>\<^sub>c \<nat>\<^sub>c \<circ>\<^sub>c left_cart_proj (\<nat>\<^sub>c \<times>\<^sub>c \<nat>\<^sub>c) \<nat>\<^sub>c,\<langle>right_cart_proj \<nat>\<^sub>c \<nat>\<^sub>c \<circ>\<^sub>c left_cart_proj (\<nat>\<^sub>c \<times>\<^sub>c \<nat>\<^sub>c) \<nat>\<^sub>c,right_cart_proj (\<nat>\<^sub>c \<times>\<^sub>c \<nat>\<^sub>c) \<nat>\<^sub>c\<rangle>\<rangle>)\<^sup>\<sharp>"
+      proof(rule one_separator[where X ="(\<nat>\<^sub>c \<times>\<^sub>c \<nat>\<^sub>c)\<times>\<^sub>c \<nat>\<^sub>c", where Y = "\<nat>\<^sub>c"])
+        show "eval_func \<nat>\<^sub>c (\<nat>\<^sub>c \<times>\<^sub>c \<nat>\<^sub>c) \<circ>\<^sub>c id\<^sub>c (\<nat>\<^sub>c \<times>\<^sub>c \<nat>\<^sub>c) \<times>\<^sub>f (mult2 \<circ>\<^sub>c (id\<^sub>c \<nat>\<^sub>c \<times>\<^sub>f mult2) \<circ>\<^sub>c \<langle>left_cart_proj \<nat>\<^sub>c \<nat>\<^sub>c \<circ>\<^sub>c left_cart_proj (\<nat>\<^sub>c \<times>\<^sub>c \<nat>\<^sub>c) \<nat>\<^sub>c,\<langle>right_cart_proj \<nat>\<^sub>c \<nat>\<^sub>c \<circ>\<^sub>c left_cart_proj (\<nat>\<^sub>c \<times>\<^sub>c \<nat>\<^sub>c) \<nat>\<^sub>c,right_cart_proj (\<nat>\<^sub>c \<times>\<^sub>c \<nat>\<^sub>c) \<nat>\<^sub>c\<rangle>\<rangle>)\<^sup>\<sharp> \<circ>\<^sub>c successor : (\<nat>\<^sub>c \<times>\<^sub>c \<nat>\<^sub>c) \<times>\<^sub>c \<nat>\<^sub>c \<rightarrow> \<nat>\<^sub>c"
+          using flat_type inv_transpose_func_def2 multIdxMultp0p0p1p0p0_SharpSucc_type by auto
+        show "eval_func \<nat>\<^sub>c (\<nat>\<^sub>c \<times>\<^sub>c \<nat>\<^sub>c) \<circ>\<^sub>c id\<^sub>c (\<nat>\<^sub>c \<times>\<^sub>c \<nat>\<^sub>c) \<times>\<^sub>f (add2 \<circ>\<^sub>c \<langle>mult2 \<circ>\<^sub>c left_cart_proj (\<nat>\<^sub>c \<times>\<^sub>c \<nat>\<^sub>c) (\<nat>\<^sub>c\<^bsup>(\<nat>\<^sub>c \<times>\<^sub>c \<nat>\<^sub>c)\<^esup>),eval_func \<nat>\<^sub>c (\<nat>\<^sub>c \<times>\<^sub>c \<nat>\<^sub>c)\<rangle>)\<^sup>\<sharp> \<circ>\<^sub>c (mult2 \<circ>\<^sub>c (id\<^sub>c \<nat>\<^sub>c \<times>\<^sub>f mult2) \<circ>\<^sub>c \<langle>left_cart_proj \<nat>\<^sub>c \<nat>\<^sub>c \<circ>\<^sub>c left_cart_proj (\<nat>\<^sub>c \<times>\<^sub>c \<nat>\<^sub>c) \<nat>\<^sub>c,\<langle>right_cart_proj \<nat>\<^sub>c \<nat>\<^sub>c \<circ>\<^sub>c left_cart_proj (\<nat>\<^sub>c \<times>\<^sub>c \<nat>\<^sub>c) \<nat>\<^sub>c,right_cart_proj (\<nat>\<^sub>c \<times>\<^sub>c \<nat>\<^sub>c) \<nat>\<^sub>c\<rangle>\<rangle>)\<^sup>\<sharp> : (\<nat>\<^sub>c \<times>\<^sub>c \<nat>\<^sub>c) \<times>\<^sub>c \<nat>\<^sub>c \<rightarrow> \<nat>\<^sub>c"
+          using flat_type inv_transpose_func_def2 type2 by auto
+        show "\<And>x. x \<in>\<^sub>c (\<nat>\<^sub>c \<times>\<^sub>c \<nat>\<^sub>c) \<times>\<^sub>c \<nat>\<^sub>c \<Longrightarrow>
+         (eval_func \<nat>\<^sub>c (\<nat>\<^sub>c \<times>\<^sub>c \<nat>\<^sub>c) \<circ>\<^sub>c id\<^sub>c (\<nat>\<^sub>c \<times>\<^sub>c \<nat>\<^sub>c) \<times>\<^sub>f (mult2 \<circ>\<^sub>c (id\<^sub>c \<nat>\<^sub>c \<times>\<^sub>f mult2) \<circ>\<^sub>c \<langle>left_cart_proj \<nat>\<^sub>c \<nat>\<^sub>c \<circ>\<^sub>c left_cart_proj (\<nat>\<^sub>c \<times>\<^sub>c \<nat>\<^sub>c) \<nat>\<^sub>c,\<langle>right_cart_proj \<nat>\<^sub>c \<nat>\<^sub>c \<circ>\<^sub>c left_cart_proj (\<nat>\<^sub>c \<times>\<^sub>c \<nat>\<^sub>c) \<nat>\<^sub>c,right_cart_proj (\<nat>\<^sub>c \<times>\<^sub>c \<nat>\<^sub>c) \<nat>\<^sub>c\<rangle>\<rangle>)\<^sup>\<sharp> \<circ>\<^sub>c successor) \<circ>\<^sub>c x =
+ (eval_func \<nat>\<^sub>c (\<nat>\<^sub>c \<times>\<^sub>c \<nat>\<^sub>c) \<circ>\<^sub>c id\<^sub>c (\<nat>\<^sub>c \<times>\<^sub>c \<nat>\<^sub>c) \<times>\<^sub>f (add2 \<circ>\<^sub>c \<langle>mult2 \<circ>\<^sub>c left_cart_proj (\<nat>\<^sub>c \<times>\<^sub>c \<nat>\<^sub>c) (\<nat>\<^sub>c\<^bsup>(\<nat>\<^sub>c \<times>\<^sub>c \<nat>\<^sub>c)\<^esup>),eval_func \<nat>\<^sub>c (\<nat>\<^sub>c \<times>\<^sub>c \<nat>\<^sub>c)\<rangle>)\<^sup>\<sharp> \<circ>\<^sub>c (mult2 \<circ>\<^sub>c (id\<^sub>c \<nat>\<^sub>c \<times>\<^sub>f mult2) \<circ>\<^sub>c \<langle>left_cart_proj \<nat>\<^sub>c \<nat>\<^sub>c \<circ>\<^sub>c left_cart_proj (\<nat>\<^sub>c \<times>\<^sub>c \<nat>\<^sub>c) \<nat>\<^sub>c,\<langle>right_cart_proj \<nat>\<^sub>c \<nat>\<^sub>c \<circ>\<^sub>c left_cart_proj (\<nat>\<^sub>c \<times>\<^sub>c \<nat>\<^sub>c) \<nat>\<^sub>c,right_cart_proj (\<nat>\<^sub>c \<times>\<^sub>c \<nat>\<^sub>c) \<nat>\<^sub>c\<rangle>\<rangle>)\<^sup>\<sharp>) \<circ>\<^sub>c x "
+        proof - 
+          fix x
+          assume x_type: "x \<in>\<^sub>c (\<nat>\<^sub>c \<times>\<^sub>c \<nat>\<^sub>c) \<times>\<^sub>c \<nat>\<^sub>c"
+          obtain y r where x_def: "y \<in>\<^sub>c (\<nat>\<^sub>c \<times>\<^sub>c \<nat>\<^sub>c) \<and> r \<in>\<^sub>c \<nat>\<^sub>c \<and> x = \<langle>y,r\<rangle>"
+            using cart_prod_decomp x_type by blast
+          obtain p q where y_def: "p  \<in>\<^sub>c \<nat>\<^sub>c \<and> q \<in>\<^sub>c \<nat>\<^sub>c \<and> y = \<langle>p,q\<rangle>"
+             using cart_prod_decomp x_def by blast
+          have pq_type: "\<langle>p,q\<rangle> \<in>\<^sub>c (\<nat>\<^sub>c \<times>\<^sub>c \<nat>\<^sub>c)"
+             using x_def y_def by force
+          have y_type: "y \<in>\<^sub>c (\<nat>\<^sub>c \<times>\<^sub>c \<nat>\<^sub>c)"
+             by (simp add: x_def)
+          have x_def2: "x = \<langle>\<langle>p,q\<rangle>,r\<rangle>"
+             using x_def y_def by blast
+          have ysr_type: "\<langle>y,successor \<circ>\<^sub>c  r\<rangle> \<in>\<^sub>c (\<nat>\<^sub>c \<times>\<^sub>c \<nat>\<^sub>c) \<times>\<^sub>c \<nat>\<^sub>c"
+            by (simp add: cfunc_prod_type succ_n_type x_def)    
+          have qsr_type: "\<langle>q,successor  \<circ>\<^sub>c r\<rangle> \<in>\<^sub>c  (\<nat>\<^sub>c \<times>\<^sub>c \<nat>\<^sub>c)"
+            by (simp add: cfunc_prod_type succ_n_type x_def y_def)
+          have qr_type: "\<langle>q,r\<rangle> \<in>\<^sub>c (\<nat>\<^sub>c \<times>\<^sub>c \<nat>\<^sub>c)"
+            by (simp add: cfunc_prod_type x_def y_def)
+          have pqr_tyep: "\<langle>p ,\<langle>q,r\<rangle>\<rangle> \<in>\<^sub>c \<nat>\<^sub>c \<times>\<^sub>c (\<nat>\<^sub>c \<times>\<^sub>c \<nat>\<^sub>c)"
+            by (simp add: cfunc_prod_type qr_type y_def)
+          have trip_shft: 
+ "\<langle>left_cart_proj \<nat>\<^sub>c \<nat>\<^sub>c \<circ>\<^sub>c left_cart_proj  (\<nat>\<^sub>c \<times>\<^sub>c \<nat>\<^sub>c) \<nat>\<^sub>c, 
+ \<langle>right_cart_proj \<nat>\<^sub>c \<nat>\<^sub>c \<circ>\<^sub>c left_cart_proj  (\<nat>\<^sub>c \<times>\<^sub>c \<nat>\<^sub>c) \<nat>\<^sub>c, 
+  right_cart_proj  (\<nat>\<^sub>c \<times>\<^sub>c \<nat>\<^sub>c) \<nat>\<^sub>c \<rangle>\<rangle> \<circ>\<^sub>c \<langle>\<langle>p,q\<rangle>,r\<rangle> = \<langle>p,\<langle>q,r\<rangle>\<rangle>"
+         
+          proof - 
+            have "\<langle>left_cart_proj \<nat>\<^sub>c \<nat>\<^sub>c \<circ>\<^sub>c left_cart_proj  (\<nat>\<^sub>c \<times>\<^sub>c \<nat>\<^sub>c) \<nat>\<^sub>c, 
+ \<langle>right_cart_proj \<nat>\<^sub>c \<nat>\<^sub>c \<circ>\<^sub>c left_cart_proj  (\<nat>\<^sub>c \<times>\<^sub>c \<nat>\<^sub>c) \<nat>\<^sub>c, 
+  right_cart_proj  (\<nat>\<^sub>c \<times>\<^sub>c \<nat>\<^sub>c) \<nat>\<^sub>c \<rangle>\<rangle> \<circ>\<^sub>c \<langle>\<langle>p,q\<rangle>,r\<rangle>  = 
+    \<langle>left_cart_proj \<nat>\<^sub>c \<nat>\<^sub>c \<circ>\<^sub>c left_cart_proj  (\<nat>\<^sub>c \<times>\<^sub>c \<nat>\<^sub>c) \<nat>\<^sub>c \<circ>\<^sub>c \<langle>\<langle>p,q\<rangle>,r\<rangle>, 
+     \<langle>right_cart_proj \<nat>\<^sub>c \<nat>\<^sub>c \<circ>\<^sub>c left_cart_proj  (\<nat>\<^sub>c \<times>\<^sub>c \<nat>\<^sub>c) \<nat>\<^sub>c, 
+      right_cart_proj  (\<nat>\<^sub>c \<times>\<^sub>c \<nat>\<^sub>c) \<nat>\<^sub>c \<rangle>\<circ>\<^sub>c \<langle>\<langle>p,q\<rangle>,r\<rangle>\<rangle>"
+              by (typecheck_cfuncs,  smt cfunc_prod_comp cfunc_type_def comp_associative x_def y_def)
+            also have "... = \<langle>p, 
+     \<langle>right_cart_proj \<nat>\<^sub>c \<nat>\<^sub>c \<circ>\<^sub>c left_cart_proj  (\<nat>\<^sub>c \<times>\<^sub>c \<nat>\<^sub>c) \<nat>\<^sub>c \<circ>\<^sub>c \<langle>\<langle>p,q\<rangle>,r\<rangle>, 
+      right_cart_proj  (\<nat>\<^sub>c \<times>\<^sub>c \<nat>\<^sub>c) \<nat>\<^sub>c \<circ>\<^sub>c \<langle>\<langle>p,q\<rangle>,r\<rangle>\<rangle>\<rangle>"
+              by (typecheck_cfuncs, smt cfunc_prod_comp comp_associative2 left_cart_proj_cfunc_prod x_def x_type y_def)
+            also have "... = \<langle>p, \<langle>q, r\<rangle>\<rangle>"
+              by (typecheck_cfuncs, metis left_cart_proj_cfunc_prod right_cart_proj_cfunc_prod x_def y_def)
+            then show ?thesis using calculation by auto
+          qed
+ obtain g where g_def: "g = (mult2 \<circ>\<^sub>c (id\<^sub>c \<nat>\<^sub>c  \<times>\<^sub>f mult2) \<circ>\<^sub>c \<langle>(left_cart_proj \<nat>\<^sub>c \<nat>\<^sub>c) \<circ>\<^sub>c (left_cart_proj (\<nat>\<^sub>c\<times>\<^sub>c \<nat>\<^sub>c) \<nat>\<^sub>c),
+\<langle>(right_cart_proj \<nat>\<^sub>c \<nat>\<^sub>c) \<circ>\<^sub>c (left_cart_proj (\<nat>\<^sub>c\<times>\<^sub>c \<nat>\<^sub>c) \<nat>\<^sub>c), (right_cart_proj (\<nat>\<^sub>c\<times>\<^sub>c \<nat>\<^sub>c) \<nat>\<^sub>c)\<rangle>\<rangle>)\<^sup>\<sharp>"
+   by simp
 
- (*Moreover,...*)
+      
 
-     have f3: "((eval_func \<nat>\<^sub>c (\<nat>\<^sub>c\<times>\<^sub>c\<nat>\<^sub>c))\<circ>\<^sub>c 
-(id\<^sub>c (\<nat>\<^sub>c\<times>\<^sub>c\<nat>\<^sub>c) \<times>\<^sub>f (zero \<circ>\<^sub>c \<beta>\<^bsub>(\<nat>\<^sub>c\<times>\<^sub>c \<nat>\<^sub>c)\<times>\<^sub>cone\<^esub>)\<^sup>\<sharp>))  \<circ>\<^sub>c \<langle>\<langle>a,b\<rangle>,id\<^sub>c one\<rangle> = zero"
-     proof - 
-       have "((eval_func \<nat>\<^sub>c (\<nat>\<^sub>c\<times>\<^sub>c\<nat>\<^sub>c))\<circ>\<^sub>c 
-(id\<^sub>c (\<nat>\<^sub>c\<times>\<^sub>c\<nat>\<^sub>c) \<times>\<^sub>f (zero \<circ>\<^sub>c \<beta>\<^bsub>(\<nat>\<^sub>c\<times>\<^sub>c \<nat>\<^sub>c)\<times>\<^sub>cone\<^esub>)\<^sup>\<sharp>))  \<circ>\<^sub>c \<langle>\<langle>a,b\<rangle>,id\<^sub>c one\<rangle> =
-(eval_func \<nat>\<^sub>c (\<nat>\<^sub>c\<times>\<^sub>c\<nat>\<^sub>c))\<circ>\<^sub>c 
-(id\<^sub>c (\<nat>\<^sub>c\<times>\<^sub>c\<nat>\<^sub>c) \<times>\<^sub>f (zero \<circ>\<^sub>c \<beta>\<^bsub>(\<nat>\<^sub>c\<times>\<^sub>c \<nat>\<^sub>c)\<times>\<^sub>cone\<^esub>)\<^sup>\<sharp>)  \<circ>\<^sub>c \<langle>\<langle>a,b\<rangle>,id\<^sub>c one\<rangle>"
-          using assms apply typecheck_cfuncs
-          using comp_associative2 by auto
-       also have "... =  (zero \<circ>\<^sub>c \<beta>\<^bsub>(\<nat>\<^sub>c\<times>\<^sub>c \<nat>\<^sub>c)\<times>\<^sub>cone\<^esub>) \<circ>\<^sub>c \<langle>\<langle>a,b\<rangle>,id\<^sub>c one\<rangle>"
-         by (metis calculation transpose_func_def zero_betaN_type)
-       also have "... = zero \<circ>\<^sub>c (\<beta>\<^bsub>(\<nat>\<^sub>c\<times>\<^sub>c \<nat>\<^sub>c)\<times>\<^sub>cone\<^esub> \<circ>\<^sub>c \<langle>\<langle>a,b\<rangle>,id\<^sub>c one\<rangle>)"
-          using assms by (typecheck_cfuncs, simp add: comp_associative2)
-       also have "... = zero"
-          using assms by (typecheck_cfuncs, metis id_right_unit2 one_unique_element)
-      then show ?thesis using calculation by auto
-qed
 
-(*Equation before "Likewise..." on page 19*)
-  have f4: "((eval_func \<nat>\<^sub>c (\<nat>\<^sub>c\<times>\<^sub>c\<nat>\<^sub>c))\<circ>\<^sub>c 
-(id\<^sub>c (\<nat>\<^sub>c\<times>\<^sub>c\<nat>\<^sub>c) \<times>\<^sub>f (mult2 \<circ>\<^sub>c (mult2 \<times>\<^sub>f id\<^sub>c \<nat>\<^sub>c))\<^sup>\<sharp>\<circ>\<^sub>c successor) )
-\<circ>\<^sub>c \<langle>\<langle>a,b\<rangle>,c\<rangle> = (a \<cdot>\<^sub>\<nat> b)  \<cdot>\<^sub>\<nat> (successor  \<circ>\<^sub>c c)"
-  proof - 
-    have "((eval_func \<nat>\<^sub>c (\<nat>\<^sub>c\<times>\<^sub>c\<nat>\<^sub>c))\<circ>\<^sub>c 
-(id\<^sub>c (\<nat>\<^sub>c\<times>\<^sub>c\<nat>\<^sub>c) \<times>\<^sub>f (mult2 \<circ>\<^sub>c (mult2 \<times>\<^sub>f id\<^sub>c \<nat>\<^sub>c))\<^sup>\<sharp>\<circ>\<^sub>c successor) )
-\<circ>\<^sub>c \<langle>\<langle>a,b\<rangle>,c\<rangle> = (eval_func \<nat>\<^sub>c (\<nat>\<^sub>c\<times>\<^sub>c\<nat>\<^sub>c))\<circ>\<^sub>c 
-(id\<^sub>c (\<nat>\<^sub>c\<times>\<^sub>c\<nat>\<^sub>c) \<times>\<^sub>f (mult2 \<circ>\<^sub>c (mult2 \<times>\<^sub>f id\<^sub>c \<nat>\<^sub>c))\<^sup>\<sharp>\<circ>\<^sub>c successor) 
-\<circ>\<^sub>c \<langle>\<langle>a,b\<rangle>,c\<rangle>"
-          using assms by (typecheck_cfuncs, simp add: comp_associative2)
-    also have "... = (eval_func \<nat>\<^sub>c (\<nat>\<^sub>c\<times>\<^sub>c\<nat>\<^sub>c))\<circ>\<^sub>c 
-(id\<^sub>c (\<nat>\<^sub>c\<times>\<^sub>c\<nat>\<^sub>c) \<times>\<^sub>f (mult2 \<circ>\<^sub>c (mult2 \<times>\<^sub>f id\<^sub>c \<nat>\<^sub>c))\<^sup>\<sharp>)\<circ>\<^sub>c (id\<^sub>c (\<nat>\<^sub>c\<times>\<^sub>c\<nat>\<^sub>c) \<times>\<^sub>f successor) 
-\<circ>\<^sub>c \<langle>\<langle>a,b\<rangle>,c\<rangle>"
-          using assms by (typecheck_cfuncs, smt comp_associative2 flat_cancels_sharp inv_transpose_func_def2 inv_transpose_of_composition)
 
-    also have "... = mult2 \<circ>\<^sub>c (mult2 \<times>\<^sub>f id\<^sub>c \<nat>\<^sub>c) \<circ>\<^sub>c (id\<^sub>c (\<nat>\<^sub>c\<times>\<^sub>c\<nat>\<^sub>c) \<times>\<^sub>f successor) \<circ>\<^sub>c \<langle>\<langle>a,b\<rangle>,c\<rangle>"
-          using assms by (typecheck_cfuncs, metis cfunc_type_def comp_associative transpose_func_def)
-    also have "... = mult2 \<circ>\<^sub>c (mult2 \<times>\<^sub>f id\<^sub>c \<nat>\<^sub>c) \<circ>\<^sub>c \<langle>id\<^sub>c (\<nat>\<^sub>c\<times>\<^sub>c\<nat>\<^sub>c)\<circ>\<^sub>c  \<langle>a,b\<rangle>,successor \<circ>\<^sub>c c\<rangle>"
-      using ab_type assms(3) cfunc_cross_prod_comp_cfunc_prod id_type successor_type by fastforce
-    also have "... = mult2 \<circ>\<^sub>c \<langle>mult2 \<circ>\<^sub>c  (id\<^sub>c (\<nat>\<^sub>c\<times>\<^sub>c\<nat>\<^sub>c)\<circ>\<^sub>c  \<langle>a,b\<rangle>),id\<^sub>c \<nat>\<^sub>c \<circ>\<^sub>c (successor \<circ>\<^sub>c c)\<rangle>"
-      using id_ab_type sc_type mult2_type id_type cfunc_cross_prod_comp_cfunc_prod by fastforce
-    also have "... =  mult2 \<circ>\<^sub>c \<langle>mult2 \<circ>\<^sub>c  (\<langle>a,b\<rangle>),(successor \<circ>\<^sub>c c)\<rangle>"
-      using ab_type id_left_unit2 sc_type by auto
-    also have "... = (a \<cdot>\<^sub>\<nat> b)  \<cdot>\<^sub>\<nat> (successor  \<circ>\<^sub>c c)"
-      by (simp add: mult_def)
-then show ?thesis using calculation by auto
-qed
+           have "(eval_func \<nat>\<^sub>c (\<nat>\<^sub>c \<times>\<^sub>c \<nat>\<^sub>c) \<circ>\<^sub>c id\<^sub>c (\<nat>\<^sub>c \<times>\<^sub>c \<nat>\<^sub>c) \<times>\<^sub>f (mult2 \<circ>\<^sub>c (id\<^sub>c \<nat>\<^sub>c \<times>\<^sub>f mult2) \<circ>\<^sub>c \<langle>left_cart_proj \<nat>\<^sub>c \<nat>\<^sub>c \<circ>\<^sub>c left_cart_proj (\<nat>\<^sub>c \<times>\<^sub>c \<nat>\<^sub>c) \<nat>\<^sub>c,\<langle>right_cart_proj \<nat>\<^sub>c \<nat>\<^sub>c \<circ>\<^sub>c left_cart_proj (\<nat>\<^sub>c \<times>\<^sub>c \<nat>\<^sub>c) \<nat>\<^sub>c,right_cart_proj (\<nat>\<^sub>c \<times>\<^sub>c \<nat>\<^sub>c) \<nat>\<^sub>c\<rangle>\<rangle>)\<^sup>\<sharp> \<circ>\<^sub>c successor) \<circ>\<^sub>c x 
+           =     (eval_func \<nat>\<^sub>c (\<nat>\<^sub>c \<times>\<^sub>c \<nat>\<^sub>c) \<circ>\<^sub>c id\<^sub>c (\<nat>\<^sub>c \<times>\<^sub>c \<nat>\<^sub>c) \<times>\<^sub>f (mult2 \<circ>\<^sub>c (id\<^sub>c \<nat>\<^sub>c \<times>\<^sub>f mult2) \<circ>\<^sub>c \<langle>left_cart_proj \<nat>\<^sub>c \<nat>\<^sub>c \<circ>\<^sub>c left_cart_proj (\<nat>\<^sub>c \<times>\<^sub>c \<nat>\<^sub>c) \<nat>\<^sub>c,\<langle>right_cart_proj \<nat>\<^sub>c \<nat>\<^sub>c \<circ>\<^sub>c left_cart_proj (\<nat>\<^sub>c \<times>\<^sub>c \<nat>\<^sub>c) \<nat>\<^sub>c,right_cart_proj (\<nat>\<^sub>c \<times>\<^sub>c \<nat>\<^sub>c) \<nat>\<^sub>c\<rangle>\<rangle>)\<^sup>\<sharp> )\<circ>\<^sub>c( (id\<^sub>c (\<nat>\<^sub>c \<times>\<^sub>c \<nat>\<^sub>c) \<times>\<^sub>f successor) \<circ>\<^sub>c x) "
+             by (typecheck_cfuncs , smt comp_associative2 inv_transpose_func_def2 inv_transpose_of_composition x_type)
+         also have "... = (mult2 \<circ>\<^sub>c (id\<^sub>c \<nat>\<^sub>c  \<times>\<^sub>f mult2) \<circ>\<^sub>c \<langle>(left_cart_proj \<nat>\<^sub>c \<nat>\<^sub>c) \<circ>\<^sub>c (left_cart_proj (\<nat>\<^sub>c\<times>\<^sub>c \<nat>\<^sub>c) \<nat>\<^sub>c),
+        \<langle>(right_cart_proj \<nat>\<^sub>c \<nat>\<^sub>c) \<circ>\<^sub>c (left_cart_proj (\<nat>\<^sub>c\<times>\<^sub>c \<nat>\<^sub>c) \<nat>\<^sub>c), (right_cart_proj (\<nat>\<^sub>c\<times>\<^sub>c \<nat>\<^sub>c) \<nat>\<^sub>c)\<rangle>\<rangle>)
+        \<circ>\<^sub>c (id\<^sub>c (\<nat>\<^sub>c\<times>\<^sub>c\<nat>\<^sub>c) \<times>\<^sub>f  successor)
+        \<circ>\<^sub>c \<langle>\<langle>p,q\<rangle>,r\<rangle>"
+           by (typecheck_cfuncs, simp add: transpose_func_def x_def2)
 
-(*Likewise ...*)
 
-  have f5: "((eval_func \<nat>\<^sub>c (\<nat>\<^sub>c\<times>\<^sub>c\<nat>\<^sub>c))\<circ>\<^sub>c 
-(id\<^sub>c (\<nat>\<^sub>c\<times>\<^sub>c\<nat>\<^sub>c) \<times>\<^sub>f ((mult2 \<circ>\<^sub>c (id\<^sub>c \<nat>\<^sub>c  \<times>\<^sub>f mult2) \<circ>\<^sub>c \<langle>(left_cart_proj \<nat>\<^sub>c \<nat>\<^sub>c) \<circ>\<^sub>c (left_cart_proj (\<nat>\<^sub>c\<times>\<^sub>c \<nat>\<^sub>c) \<nat>\<^sub>c),
-\<langle>(right_cart_proj \<nat>\<^sub>c \<nat>\<^sub>c) \<circ>\<^sub>c (left_cart_proj (\<nat>\<^sub>c\<times>\<^sub>c \<nat>\<^sub>c) \<nat>\<^sub>c), (right_cart_proj (\<nat>\<^sub>c\<times>\<^sub>c \<nat>\<^sub>c) \<nat>\<^sub>c)\<rangle>\<rangle>)\<^sup>\<sharp> \<circ>\<^sub>c successor)))
-\<circ>\<^sub>c \<langle>\<langle>a,b\<rangle>,c\<rangle> = a \<cdot>\<^sub>\<nat> (b  \<cdot>\<^sub>\<nat> (successor  \<circ>\<^sub>c c))"
-  proof - 
-    have "((eval_func \<nat>\<^sub>c (\<nat>\<^sub>c\<times>\<^sub>c\<nat>\<^sub>c))\<circ>\<^sub>c 
-(id\<^sub>c (\<nat>\<^sub>c\<times>\<^sub>c\<nat>\<^sub>c) \<times>\<^sub>f ((mult2 \<circ>\<^sub>c (id\<^sub>c \<nat>\<^sub>c  \<times>\<^sub>f mult2) \<circ>\<^sub>c \<langle>(left_cart_proj \<nat>\<^sub>c \<nat>\<^sub>c) \<circ>\<^sub>c (left_cart_proj (\<nat>\<^sub>c\<times>\<^sub>c \<nat>\<^sub>c) \<nat>\<^sub>c),
-\<langle>(right_cart_proj \<nat>\<^sub>c \<nat>\<^sub>c) \<circ>\<^sub>c (left_cart_proj (\<nat>\<^sub>c\<times>\<^sub>c \<nat>\<^sub>c) \<nat>\<^sub>c), (right_cart_proj (\<nat>\<^sub>c\<times>\<^sub>c \<nat>\<^sub>c) \<nat>\<^sub>c)\<rangle>\<rangle>)\<^sup>\<sharp> \<circ>\<^sub>c successor)))
-\<circ>\<^sub>c \<langle>\<langle>a,b\<rangle>,c\<rangle> =(eval_func \<nat>\<^sub>c (\<nat>\<^sub>c\<times>\<^sub>c\<nat>\<^sub>c))\<circ>\<^sub>c 
-(id\<^sub>c (\<nat>\<^sub>c\<times>\<^sub>c\<nat>\<^sub>c) \<times>\<^sub>f ((mult2 \<circ>\<^sub>c (id\<^sub>c \<nat>\<^sub>c  \<times>\<^sub>f mult2) \<circ>\<^sub>c \<langle>(left_cart_proj \<nat>\<^sub>c \<nat>\<^sub>c) \<circ>\<^sub>c (left_cart_proj (\<nat>\<^sub>c\<times>\<^sub>c \<nat>\<^sub>c) \<nat>\<^sub>c),
-\<langle>(right_cart_proj \<nat>\<^sub>c \<nat>\<^sub>c) \<circ>\<^sub>c (left_cart_proj (\<nat>\<^sub>c\<times>\<^sub>c \<nat>\<^sub>c) \<nat>\<^sub>c), (right_cart_proj (\<nat>\<^sub>c\<times>\<^sub>c \<nat>\<^sub>c) \<nat>\<^sub>c)\<rangle>\<rangle>)\<^sup>\<sharp> \<circ>\<^sub>c successor))
-\<circ>\<^sub>c \<langle>\<langle>a,b\<rangle>,c\<rangle>"
-          using assms by (typecheck_cfuncs, simp add: comp_associative2)
-     also have "... = (eval_func \<nat>\<^sub>c (\<nat>\<^sub>c\<times>\<^sub>c\<nat>\<^sub>c))\<circ>\<^sub>c 
-(id\<^sub>c (\<nat>\<^sub>c\<times>\<^sub>c\<nat>\<^sub>c) \<times>\<^sub>f ((mult2 \<circ>\<^sub>c (id\<^sub>c \<nat>\<^sub>c  \<times>\<^sub>f mult2) \<circ>\<^sub>c \<langle>(left_cart_proj \<nat>\<^sub>c \<nat>\<^sub>c) \<circ>\<^sub>c (left_cart_proj (\<nat>\<^sub>c\<times>\<^sub>c \<nat>\<^sub>c) \<nat>\<^sub>c),
-\<langle>(right_cart_proj \<nat>\<^sub>c \<nat>\<^sub>c) \<circ>\<^sub>c (left_cart_proj (\<nat>\<^sub>c\<times>\<^sub>c \<nat>\<^sub>c) \<nat>\<^sub>c), (right_cart_proj (\<nat>\<^sub>c\<times>\<^sub>c \<nat>\<^sub>c) \<nat>\<^sub>c)\<rangle>\<rangle>)\<^sup>\<sharp>))
-\<circ>\<^sub>c (id\<^sub>c (\<nat>\<^sub>c\<times>\<^sub>c\<nat>\<^sub>c) \<times>\<^sub>f  successor)
-\<circ>\<^sub>c \<langle>\<langle>a,b\<rangle>,c\<rangle>"
-           using assms by (typecheck_cfuncs, smt comp_associative2 flat_cancels_sharp inv_transpose_func_def2 inv_transpose_of_composition)
     also have "... = (mult2 \<circ>\<^sub>c (id\<^sub>c \<nat>\<^sub>c  \<times>\<^sub>f mult2) \<circ>\<^sub>c \<langle>(left_cart_proj \<nat>\<^sub>c \<nat>\<^sub>c) \<circ>\<^sub>c (left_cart_proj (\<nat>\<^sub>c\<times>\<^sub>c \<nat>\<^sub>c) \<nat>\<^sub>c),
 \<langle>(right_cart_proj \<nat>\<^sub>c \<nat>\<^sub>c) \<circ>\<^sub>c (left_cart_proj (\<nat>\<^sub>c\<times>\<^sub>c \<nat>\<^sub>c) \<nat>\<^sub>c), (right_cart_proj (\<nat>\<^sub>c\<times>\<^sub>c \<nat>\<^sub>c) \<nat>\<^sub>c)\<rangle>\<rangle>)
-\<circ>\<^sub>c (id\<^sub>c (\<nat>\<^sub>c\<times>\<^sub>c\<nat>\<^sub>c) \<times>\<^sub>f  successor)
-\<circ>\<^sub>c \<langle>\<langle>a,b\<rangle>,c\<rangle>"
-          using assms by (typecheck_cfuncs, smt comp_associative2 transpose_func_def)
+\<circ>\<^sub>c \<langle>id\<^sub>c (\<nat>\<^sub>c\<times>\<^sub>c\<nat>\<^sub>c) \<circ>\<^sub>c \<langle>p,q\<rangle>,successor  \<circ>\<^sub>c r\<rangle>"
+      by (typecheck_cfuncs , smt cfunc_cross_prod_comp_cfunc_prod x_def y_def)
+
+
     also have "... = (mult2 \<circ>\<^sub>c (id\<^sub>c \<nat>\<^sub>c  \<times>\<^sub>f mult2) \<circ>\<^sub>c \<langle>(left_cart_proj \<nat>\<^sub>c \<nat>\<^sub>c) \<circ>\<^sub>c (left_cart_proj (\<nat>\<^sub>c\<times>\<^sub>c \<nat>\<^sub>c) \<nat>\<^sub>c),
 \<langle>(right_cart_proj \<nat>\<^sub>c \<nat>\<^sub>c) \<circ>\<^sub>c (left_cart_proj (\<nat>\<^sub>c\<times>\<^sub>c \<nat>\<^sub>c) \<nat>\<^sub>c), (right_cart_proj (\<nat>\<^sub>c\<times>\<^sub>c \<nat>\<^sub>c) \<nat>\<^sub>c)\<rangle>\<rangle>)
-\<circ>\<^sub>c \<langle>id\<^sub>c (\<nat>\<^sub>c\<times>\<^sub>c\<nat>\<^sub>c) \<circ>\<^sub>c \<langle>a,b\<rangle>,successor  \<circ>\<^sub>c c\<rangle>"
-      using ab_type assms(3) cfunc_cross_prod_comp_cfunc_prod id_type successor_type by fastforce
-    also have "... = (mult2 \<circ>\<^sub>c (id\<^sub>c \<nat>\<^sub>c  \<times>\<^sub>f mult2) \<circ>\<^sub>c \<langle>(left_cart_proj \<nat>\<^sub>c \<nat>\<^sub>c) \<circ>\<^sub>c (left_cart_proj (\<nat>\<^sub>c\<times>\<^sub>c \<nat>\<^sub>c) \<nat>\<^sub>c),
-\<langle>(right_cart_proj \<nat>\<^sub>c \<nat>\<^sub>c) \<circ>\<^sub>c (left_cart_proj (\<nat>\<^sub>c\<times>\<^sub>c \<nat>\<^sub>c) \<nat>\<^sub>c), (right_cart_proj (\<nat>\<^sub>c\<times>\<^sub>c \<nat>\<^sub>c) \<nat>\<^sub>c)\<rangle>\<rangle>)
-\<circ>\<^sub>c \<langle>\<langle>a,b\<rangle>,successor  \<circ>\<^sub>c c\<rangle>"
-      using ab_type id_left_unit2 by auto
+\<circ>\<^sub>c \<langle>\<langle>p,q\<rangle>,successor  \<circ>\<^sub>c r\<rangle>"
+      by (typecheck_cfuncs, metis id_left_unit2 y_def)
+
     also have "... = mult2 \<circ>\<^sub>c (id\<^sub>c \<nat>\<^sub>c  \<times>\<^sub>f mult2) \<circ>\<^sub>c \<langle>(left_cart_proj \<nat>\<^sub>c \<nat>\<^sub>c) \<circ>\<^sub>c (left_cart_proj (\<nat>\<^sub>c\<times>\<^sub>c \<nat>\<^sub>c) \<nat>\<^sub>c),
 \<langle>(right_cart_proj \<nat>\<^sub>c \<nat>\<^sub>c) \<circ>\<^sub>c (left_cart_proj (\<nat>\<^sub>c\<times>\<^sub>c \<nat>\<^sub>c) \<nat>\<^sub>c), (right_cart_proj (\<nat>\<^sub>c\<times>\<^sub>c \<nat>\<^sub>c) \<nat>\<^sub>c)\<rangle>\<rangle>
-\<circ>\<^sub>c \<langle>\<langle>a,b\<rangle>,successor  \<circ>\<^sub>c c\<rangle>"
-          using assms by (typecheck_cfuncs, simp add: comp_associative2)
-          
-    also have "... = mult2 \<circ>\<^sub>c (id\<^sub>c \<nat>\<^sub>c  \<times>\<^sub>f mult2) \<circ>\<^sub>c \<langle>(left_cart_proj \<nat>\<^sub>c \<nat>\<^sub>c) \<circ>\<^sub>c (left_cart_proj (\<nat>\<^sub>c\<times>\<^sub>c \<nat>\<^sub>c) \<nat>\<^sub>c)\<circ>\<^sub>c \<langle>\<langle>a,b\<rangle>,successor  \<circ>\<^sub>c c\<rangle> ,
-\<langle>(right_cart_proj \<nat>\<^sub>c \<nat>\<^sub>c) \<circ>\<^sub>c (left_cart_proj (\<nat>\<^sub>c\<times>\<^sub>c \<nat>\<^sub>c) \<nat>\<^sub>c), (right_cart_proj (\<nat>\<^sub>c\<times>\<^sub>c \<nat>\<^sub>c) \<nat>\<^sub>c)\<rangle>    \<circ>\<^sub>c \<langle>\<langle>a,b\<rangle>,successor  \<circ>\<^sub>c c\<rangle>   \<rangle>"
-          using assms by (typecheck_cfuncs, simp add: cfunc_prod_comp comp_associative2)
-    also have "... = mult2 \<circ>\<^sub>c (id\<^sub>c \<nat>\<^sub>c  \<times>\<^sub>f mult2) \<circ>\<^sub>c \<langle>(left_cart_proj \<nat>\<^sub>c \<nat>\<^sub>c) \<circ>\<^sub>c \<langle>a,b\<rangle> ,
-\<langle>(right_cart_proj \<nat>\<^sub>c \<nat>\<^sub>c) \<circ>\<^sub>c (left_cart_proj (\<nat>\<^sub>c\<times>\<^sub>c \<nat>\<^sub>c) \<nat>\<^sub>c)\<circ>\<^sub>c \<langle>\<langle>a,b\<rangle>,successor  \<circ>\<^sub>c c\<rangle>  , (right_cart_proj (\<nat>\<^sub>c\<times>\<^sub>c \<nat>\<^sub>c) \<nat>\<^sub>c) \<circ>\<^sub>c \<langle>\<langle>a,b\<rangle>,successor  \<circ>\<^sub>c c\<rangle>\<rangle>\<rangle>"
-          using assms by (typecheck_cfuncs, smt cfunc_prod_comp comp_associative2 left_cart_proj_cfunc_prod)
-    also have "... = mult2 \<circ>\<^sub>c (id\<^sub>c \<nat>\<^sub>c  \<times>\<^sub>f mult2) \<circ>\<^sub>c \<langle>a ,
-\<langle>(right_cart_proj \<nat>\<^sub>c \<nat>\<^sub>c) \<circ>\<^sub>c \<langle>a,b\<rangle>  , successor  \<circ>\<^sub>c c  \<rangle>  \<rangle>"
-      using ab_type assms(1) assms(2) left_cart_proj_cfunc_prod right_cart_proj_cfunc_prod sc_type by auto
-    also have "... = mult2 \<circ>\<^sub>c (id\<^sub>c \<nat>\<^sub>c  \<times>\<^sub>f mult2) \<circ>\<^sub>c \<langle>a,\<langle>b,successor  \<circ>\<^sub>c c\<rangle>\<rangle>"
-      using assms(1) assms(2) right_cart_proj_cfunc_prod by auto
-    also have "... = mult2 \<circ>\<^sub>c  \<langle>id\<^sub>c \<nat>\<^sub>c \<circ>\<^sub>c a, mult2 \<circ>\<^sub>c \<langle>b,successor  \<circ>\<^sub>c c\<rangle>\<rangle>"
-      using assms(1) bSc_type id_type mult2_type cfunc_cross_prod_comp_cfunc_prod by fastforce
-    also have "... =   a \<cdot>\<^sub>\<nat> (b  \<cdot>\<^sub>\<nat> (successor  \<circ>\<^sub>c c))"
-      using assms(1) id_left_unit2 mult_def by auto
-then show ?thesis using calculation by auto
+\<circ>\<^sub>c \<langle>\<langle>p,q\<rangle>,successor  \<circ>\<^sub>c r\<rangle>"
+      using cfunc_type_def comp_associative y_def ysr_type by (typecheck_cfuncs, fastforce)
+
+    also have "... = mult2 \<circ>\<^sub>c (id\<^sub>c \<nat>\<^sub>c  \<times>\<^sub>f mult2) \<circ>\<^sub>c \<langle>(left_cart_proj \<nat>\<^sub>c \<nat>\<^sub>c) \<circ>\<^sub>c (left_cart_proj (\<nat>\<^sub>c\<times>\<^sub>c \<nat>\<^sub>c) \<nat>\<^sub>c)\<circ>\<^sub>c \<langle>\<langle>p,q\<rangle>,successor  \<circ>\<^sub>c r\<rangle> ,
+\<langle>(right_cart_proj \<nat>\<^sub>c \<nat>\<^sub>c) \<circ>\<^sub>c (left_cart_proj (\<nat>\<^sub>c\<times>\<^sub>c \<nat>\<^sub>c) \<nat>\<^sub>c), (right_cart_proj (\<nat>\<^sub>c\<times>\<^sub>c \<nat>\<^sub>c) \<nat>\<^sub>c)\<rangle>    \<circ>\<^sub>c \<langle>\<langle>p,q\<rangle>,successor  \<circ>\<^sub>c r\<rangle>   \<rangle>"
+      by (typecheck_cfuncs, smt cfunc_prod_comp cfunc_type_def comp_associative y_def ysr_type)
+
+    also have "... = mult2 \<circ>\<^sub>c (id\<^sub>c \<nat>\<^sub>c  \<times>\<^sub>f mult2) \<circ>\<^sub>c \<langle>(left_cart_proj \<nat>\<^sub>c \<nat>\<^sub>c) \<circ>\<^sub>c \<langle>p,q\<rangle> ,
+\<langle>(right_cart_proj \<nat>\<^sub>c \<nat>\<^sub>c) \<circ>\<^sub>c (left_cart_proj (\<nat>\<^sub>c\<times>\<^sub>c \<nat>\<^sub>c) \<nat>\<^sub>c)\<circ>\<^sub>c \<langle>\<langle>p,q\<rangle>,successor  \<circ>\<^sub>c r\<rangle>  , (right_cart_proj (\<nat>\<^sub>c\<times>\<^sub>c \<nat>\<^sub>c) \<nat>\<^sub>c) \<circ>\<^sub>c \<langle>\<langle>p,q\<rangle>,successor  \<circ>\<^sub>c r\<rangle>\<rangle>\<rangle>"
+      by (typecheck_cfuncs, smt cfunc_prod_comp comp_associative2 left_cart_proj_cfunc_prod x_def y_def ysr_type)
+
+    
+   also have "... = mult2 \<circ>\<^sub>c (id\<^sub>c \<nat>\<^sub>c  \<times>\<^sub>f mult2) \<circ>\<^sub>c \<langle>p ,
+\<langle>(right_cart_proj \<nat>\<^sub>c \<nat>\<^sub>c) \<circ>\<^sub>c \<langle>p,q\<rangle>  , successor  \<circ>\<^sub>c r  \<rangle>  \<rangle>"
+     by (typecheck_cfuncs, smt left_cart_proj_cfunc_prod right_cart_proj_cfunc_prod x_def y_def)    
+
+    
+     also have "... = mult2 \<circ>\<^sub>c (id\<^sub>c \<nat>\<^sub>c  \<times>\<^sub>f mult2) \<circ>\<^sub>c \<langle>p,\<langle>q,successor  \<circ>\<^sub>c r\<rangle>\<rangle>"
+       by (typecheck_cfuncs, metis right_cart_proj_cfunc_prod y_def)
+
+    also have "... = mult2 \<circ>\<^sub>c  \<langle>id\<^sub>c \<nat>\<^sub>c \<circ>\<^sub>c p, mult2 \<circ>\<^sub>c \<langle>q,successor  \<circ>\<^sub>c r\<rangle>\<rangle>"
+      using cfunc_cross_prod_comp_cfunc_prod qsr_type y_def by (typecheck_cfuncs, auto)
+
+    also have "... =   p \<cdot>\<^sub>\<nat> (q  \<cdot>\<^sub>\<nat> (successor  \<circ>\<^sub>c r))"
+      using id_left_unit2 mult_def y_def by (typecheck_cfuncs, auto)
+
+    also have "... = (q  \<cdot>\<^sub>\<nat> (successor  \<circ>\<^sub>c r))  \<cdot>\<^sub>\<nat> p"
+      by (simp add: mult_closure mult_commutative succ_n_type x_def y_def)
+
+    also have "... = (q +\<^sub>\<nat> (q \<cdot>\<^sub>\<nat> r)) \<cdot>\<^sub>\<nat> p"
+      by (simp add: mult_respects_succ_right x_def y_def)
+
+    also have "... = (q \<cdot>\<^sub>\<nat> p) +\<^sub>\<nat> ((q \<cdot>\<^sub>\<nat> r) \<cdot>\<^sub>\<nat> p)"
+      by (simp add: mult_Left_Distributivity mult_closure x_def y_def)
+
+    also have "... = (p \<cdot>\<^sub>\<nat> q) +\<^sub>\<nat> (p \<cdot>\<^sub>\<nat> (q \<cdot>\<^sub>\<nat> r))"
+      by (simp add: mult_closure mult_commutative x_def y_def)
+
+    also have "... = add2 \<circ>\<^sub>c \<langle>(p \<cdot>\<^sub>\<nat> q), (p \<cdot>\<^sub>\<nat> (q \<cdot>\<^sub>\<nat> r))\<rangle>"
+      by (simp add: add_def)
+
+    also have "... = add2 \<circ>\<^sub>c \<langle>mult2 \<circ>\<^sub>c \<langle>p,q\<rangle>, mult2\<circ>\<^sub>c \<langle>p , mult2\<circ>\<^sub>c\<langle>q,r\<rangle>\<rangle>\<rangle>"
+      by (simp add: mult_def)
+
+    also have "... = add2 \<circ>\<^sub>c \<langle>mult2 \<circ>\<^sub>c (left_cart_proj (\<nat>\<^sub>c\<times>\<^sub>c \<nat>\<^sub>c) \<nat>\<^sub>c) \<circ>\<^sub>c \<langle>\<langle>p,q\<rangle>,r\<rangle>, 
+                              mult2\<circ>\<^sub>c \<langle>id \<nat>\<^sub>c \<circ>\<^sub>c  p , mult2\<circ>\<^sub>c\<langle>q,r\<rangle>\<rangle>\<rangle>"
+      by(typecheck_cfuncs, metis id_left_unit2 left_cart_proj_cfunc_prod x_def y_def)
+
+    also have "... = add2 \<circ>\<^sub>c \<langle>mult2 \<circ>\<^sub>c (left_cart_proj (\<nat>\<^sub>c\<times>\<^sub>c \<nat>\<^sub>c) \<nat>\<^sub>c) \<circ>\<^sub>c x, 
+                              mult2\<circ>\<^sub>c (id \<nat>\<^sub>c \<times>\<^sub>f mult2) \<circ>\<^sub>c \<langle>p ,\<langle>q,r\<rangle>\<rangle>\<rangle>"
+      using cfunc_cross_prod_comp_cfunc_prod qr_type x_def y_def by (typecheck_cfuncs, auto)
+
+    also have "... = add2 \<circ>\<^sub>c \<langle>mult2 \<circ>\<^sub>c (left_cart_proj (\<nat>\<^sub>c\<times>\<^sub>c \<nat>\<^sub>c) \<nat>\<^sub>c) \<circ>\<^sub>c x, 
+                              mult2\<circ>\<^sub>c (id \<nat>\<^sub>c \<times>\<^sub>f mult2) \<circ>\<^sub>c 
+\<langle>left_cart_proj \<nat>\<^sub>c \<nat>\<^sub>c \<circ>\<^sub>c
+   left_cart_proj (\<nat>\<^sub>c \<times>\<^sub>c \<nat>\<^sub>c)
+    \<nat>\<^sub>c,\<langle>right_cart_proj \<nat>\<^sub>c \<nat>\<^sub>c \<circ>\<^sub>c
+         left_cart_proj (\<nat>\<^sub>c \<times>\<^sub>c \<nat>\<^sub>c) \<nat>\<^sub>c,right_cart_proj (\<nat>\<^sub>c \<times>\<^sub>c \<nat>\<^sub>c) \<nat>\<^sub>c\<rangle>\<rangle> \<circ>\<^sub>c
+  \<langle>\<langle>p,q\<rangle>,r\<rangle>\<rangle>"
+      by (simp add: trip_shft)
+    also have "... = add2 \<circ>\<^sub>c \<langle>(mult2 \<circ>\<^sub>c id (\<nat>\<^sub>c \<times>\<^sub>c \<nat>\<^sub>c)  \<circ>\<^sub>c  left_cart_proj (\<nat>\<^sub>c\<times>\<^sub>c \<nat>\<^sub>c) \<nat>\<^sub>c) \<circ>\<^sub>c x, 
+                              mult2\<circ>\<^sub>c (id \<nat>\<^sub>c \<times>\<^sub>f mult2) \<circ>\<^sub>c 
+\<langle>left_cart_proj \<nat>\<^sub>c \<nat>\<^sub>c \<circ>\<^sub>c
+   left_cart_proj (\<nat>\<^sub>c \<times>\<^sub>c \<nat>\<^sub>c)
+    \<nat>\<^sub>c,\<langle>right_cart_proj \<nat>\<^sub>c \<nat>\<^sub>c \<circ>\<^sub>c
+         left_cart_proj (\<nat>\<^sub>c \<times>\<^sub>c \<nat>\<^sub>c) \<nat>\<^sub>c,right_cart_proj (\<nat>\<^sub>c \<times>\<^sub>c \<nat>\<^sub>c) \<nat>\<^sub>c\<rangle>\<rangle> \<circ>\<^sub>c
+  x\<rangle>"
+      using cfunc_type_def comp_associative id_left_unit2 x_def y_def by (typecheck_cfuncs, auto)
+
+
+also have "... = add2 \<circ>\<^sub>c \<langle>mult2 \<circ>\<^sub>c (id (\<nat>\<^sub>c \<times>\<^sub>c \<nat>\<^sub>c)  \<circ>\<^sub>c  left_cart_proj (\<nat>\<^sub>c\<times>\<^sub>c \<nat>\<^sub>c) \<nat>\<^sub>c) , 
+                              mult2\<circ>\<^sub>c (id \<nat>\<^sub>c \<times>\<^sub>f mult2) \<circ>\<^sub>c 
+\<langle>left_cart_proj \<nat>\<^sub>c \<nat>\<^sub>c \<circ>\<^sub>c
+   left_cart_proj (\<nat>\<^sub>c \<times>\<^sub>c \<nat>\<^sub>c)
+    \<nat>\<^sub>c,\<langle>right_cart_proj \<nat>\<^sub>c \<nat>\<^sub>c \<circ>\<^sub>c
+         left_cart_proj (\<nat>\<^sub>c \<times>\<^sub>c \<nat>\<^sub>c) \<nat>\<^sub>c,right_cart_proj (\<nat>\<^sub>c \<times>\<^sub>c \<nat>\<^sub>c) \<nat>\<^sub>c\<rangle>\<rangle> \<rangle> \<circ>\<^sub>c x"
+  by (typecheck_cfuncs, smt cfunc_prod_comp comp_associative2 x_type)
+
+also have "... = add2 \<circ>\<^sub>c \<langle>mult2 \<circ>\<^sub>c (left_cart_proj (\<nat>\<^sub>c\<times>\<^sub>c \<nat>\<^sub>c) (\<nat>\<^sub>c\<^bsup>(\<nat>\<^sub>c \<times>\<^sub>c \<nat>\<^sub>c)\<^esup>) \<circ>\<^sub>c (id (\<nat>\<^sub>c\<times>\<^sub>c \<nat>\<^sub>c) \<times>\<^sub>f g)  ) , 
+                              mult2\<circ>\<^sub>c (id \<nat>\<^sub>c \<times>\<^sub>f mult2) \<circ>\<^sub>c 
+\<langle>left_cart_proj \<nat>\<^sub>c \<nat>\<^sub>c \<circ>\<^sub>c
+   left_cart_proj (\<nat>\<^sub>c \<times>\<^sub>c \<nat>\<^sub>c)
+    \<nat>\<^sub>c,\<langle>right_cart_proj \<nat>\<^sub>c \<nat>\<^sub>c \<circ>\<^sub>c
+         left_cart_proj (\<nat>\<^sub>c \<times>\<^sub>c \<nat>\<^sub>c) \<nat>\<^sub>c,right_cart_proj (\<nat>\<^sub>c \<times>\<^sub>c \<nat>\<^sub>c) \<nat>\<^sub>c\<rangle>\<rangle> \<rangle> \<circ>\<^sub>c x"
+  using g_def left_cart_proj_cfunc_cross_prod multIdxMultp0p0p1p0p1_Sharp_type by (typecheck_cfuncs, auto)
+
+  also have "... = add2 \<circ>\<^sub>c \<langle>mult2 \<circ>\<^sub>c (left_cart_proj (\<nat>\<^sub>c\<times>\<^sub>c \<nat>\<^sub>c) (\<nat>\<^sub>c\<^bsup>(\<nat>\<^sub>c \<times>\<^sub>c \<nat>\<^sub>c)\<^esup>) \<circ>\<^sub>c (id (\<nat>\<^sub>c\<times>\<^sub>c \<nat>\<^sub>c) \<times>\<^sub>f g)  ) , 
+                             eval_func \<nat>\<^sub>c (\<nat>\<^sub>c \<times>\<^sub>c \<nat>\<^sub>c) \<circ>\<^sub>c (id (\<nat>\<^sub>c\<times>\<^sub>c \<nat>\<^sub>c) \<times>\<^sub>f g)   \<rangle> \<circ>\<^sub>c x"
+    using g_def transpose_func_def by (typecheck_cfuncs, auto)
+
+  also have "... = ((add2 \<circ>\<^sub>c 
+\<langle>mult2 \<circ>\<^sub>c (left_cart_proj (\<nat>\<^sub>c\<times>\<^sub>c \<nat>\<^sub>c) (\<nat>\<^sub>c\<^bsup>(\<nat>\<^sub>c \<times>\<^sub>c \<nat>\<^sub>c)\<^esup>)   ) , 
+                             eval_func \<nat>\<^sub>c (\<nat>\<^sub>c \<times>\<^sub>c \<nat>\<^sub>c)   \<rangle>)
+ \<circ>\<^sub>c (id (\<nat>\<^sub>c\<times>\<^sub>c \<nat>\<^sub>c) \<times>\<^sub>f g)) \<circ>\<^sub>c x"
+    by (typecheck_cfuncs, smt cfunc_prod_comp cfunc_type_def comp_associative g_def multIdxMultp0p0p1p0p1_Sharp_type x_type)
+
+  also have "... = (
+(eval_func \<nat>\<^sub>c (\<nat>\<^sub>c \<times>\<^sub>c \<nat>\<^sub>c) \<circ>\<^sub>c id\<^sub>c (\<nat>\<^sub>c \<times>\<^sub>c \<nat>\<^sub>c) \<times>\<^sub>f 
+(add2 \<circ>\<^sub>c
+\<langle>mult2 \<circ>\<^sub>c (left_cart_proj (\<nat>\<^sub>c\<times>\<^sub>c \<nat>\<^sub>c) (\<nat>\<^sub>c\<^bsup>(\<nat>\<^sub>c \<times>\<^sub>c \<nat>\<^sub>c)\<^esup>)   ) , 
+                             eval_func \<nat>\<^sub>c (\<nat>\<^sub>c \<times>\<^sub>c \<nat>\<^sub>c)   \<rangle>)\<^sup>\<sharp>)
+ \<circ>\<^sub>c (id (\<nat>\<^sub>c\<times>\<^sub>c \<nat>\<^sub>c) \<times>\<^sub>f g)) \<circ>\<^sub>c x"
+    by (typecheck_cfuncs, simp add: transpose_func_def)
+
+  also have "... = 
+(eval_func \<nat>\<^sub>c (\<nat>\<^sub>c \<times>\<^sub>c \<nat>\<^sub>c) \<circ>\<^sub>c ( id\<^sub>c (\<nat>\<^sub>c \<times>\<^sub>c \<nat>\<^sub>c) \<times>\<^sub>f 
+(add2 \<circ>\<^sub>c
+\<langle>mult2 \<circ>\<^sub>c (left_cart_proj (\<nat>\<^sub>c\<times>\<^sub>c \<nat>\<^sub>c) (\<nat>\<^sub>c\<^bsup>(\<nat>\<^sub>c \<times>\<^sub>c \<nat>\<^sub>c)\<^esup>)   ) , 
+                             eval_func \<nat>\<^sub>c (\<nat>\<^sub>c \<times>\<^sub>c \<nat>\<^sub>c)   \<rangle>)\<^sup>\<sharp>)
+ \<circ>\<^sub>c id (\<nat>\<^sub>c\<times>\<^sub>c \<nat>\<^sub>c) \<times>\<^sub>f g) \<circ>\<^sub>c x" 
+    by (typecheck_cfuncs, smt g_def identity_distributes_across_composition inv_transpose_func_def2 inv_transpose_of_composition multIdxMultp0p0p1p0p1_Sharp_type type2)
+
+also have "... = 
+eval_func \<nat>\<^sub>c (\<nat>\<^sub>c \<times>\<^sub>c \<nat>\<^sub>c) \<circ>\<^sub>c (
+( id\<^sub>c (\<nat>\<^sub>c \<times>\<^sub>c \<nat>\<^sub>c) \<times>\<^sub>f
+(add2 \<circ>\<^sub>c
+\<langle>mult2 \<circ>\<^sub>c (left_cart_proj (\<nat>\<^sub>c\<times>\<^sub>c \<nat>\<^sub>c) (\<nat>\<^sub>c\<^bsup>(\<nat>\<^sub>c \<times>\<^sub>c \<nat>\<^sub>c)\<^esup>)   ) , 
+                             eval_func \<nat>\<^sub>c (\<nat>\<^sub>c \<times>\<^sub>c \<nat>\<^sub>c)   \<rangle>)\<^sup>\<sharp>)
+ \<circ>\<^sub>c (id (\<nat>\<^sub>c\<times>\<^sub>c \<nat>\<^sub>c) \<times>\<^sub>f g)) \<circ>\<^sub>c x"  
+  by (typecheck_cfuncs, smt comp_associative2 g_def multIdxMultp0p0p1p0p1_Sharp_type x_type)
+
+also have "... = 
+(eval_func \<nat>\<^sub>c (\<nat>\<^sub>c \<times>\<^sub>c \<nat>\<^sub>c) \<circ>\<^sub>c 
+( id\<^sub>c (\<nat>\<^sub>c \<times>\<^sub>c \<nat>\<^sub>c) \<times>\<^sub>f
+(add2 \<circ>\<^sub>c
+\<langle>mult2 \<circ>\<^sub>c (left_cart_proj (\<nat>\<^sub>c\<times>\<^sub>c \<nat>\<^sub>c) (\<nat>\<^sub>c\<^bsup>(\<nat>\<^sub>c \<times>\<^sub>c \<nat>\<^sub>c)\<^esup>)   ) , 
+                             eval_func \<nat>\<^sub>c (\<nat>\<^sub>c \<times>\<^sub>c \<nat>\<^sub>c)   \<rangle>)\<^sup>\<sharp>)
+ \<circ>\<^sub>c (id (\<nat>\<^sub>c\<times>\<^sub>c \<nat>\<^sub>c) \<times>\<^sub>f g)) \<circ>\<^sub>c x"  
+  by (simp add: \<open>(eval_func \<nat>\<^sub>c (\<nat>\<^sub>c \<times>\<^sub>c \<nat>\<^sub>c) \<circ>\<^sub>c (id\<^sub>c (\<nat>\<^sub>c \<times>\<^sub>c \<nat>\<^sub>c) \<times>\<^sub>f (add2 \<circ>\<^sub>c \<langle>mult2 \<circ>\<^sub>c left_cart_proj (\<nat>\<^sub>c \<times>\<^sub>c \<nat>\<^sub>c) (\<nat>\<^sub>c\<^bsup>(\<nat>\<^sub>c \<times>\<^sub>c \<nat>\<^sub>c)\<^esup>),eval_func \<nat>\<^sub>c (\<nat>\<^sub>c \<times>\<^sub>c \<nat>\<^sub>c)\<rangle>)\<^sup>\<sharp>) \<circ>\<^sub>c id\<^sub>c (\<nat>\<^sub>c \<times>\<^sub>c \<nat>\<^sub>c) \<times>\<^sub>f g) \<circ>\<^sub>c x = eval_func \<nat>\<^sub>c (\<nat>\<^sub>c \<times>\<^sub>c \<nat>\<^sub>c) \<circ>\<^sub>c ((id\<^sub>c (\<nat>\<^sub>c \<times>\<^sub>c \<nat>\<^sub>c) \<times>\<^sub>f (add2 \<circ>\<^sub>c \<langle>mult2 \<circ>\<^sub>c left_cart_proj (\<nat>\<^sub>c \<times>\<^sub>c \<nat>\<^sub>c) (\<nat>\<^sub>c\<^bsup>(\<nat>\<^sub>c \<times>\<^sub>c \<nat>\<^sub>c)\<^esup>),eval_func \<nat>\<^sub>c (\<nat>\<^sub>c \<times>\<^sub>c \<nat>\<^sub>c)\<rangle>)\<^sup>\<sharp>) \<circ>\<^sub>c id\<^sub>c (\<nat>\<^sub>c \<times>\<^sub>c \<nat>\<^sub>c) \<times>\<^sub>f g) \<circ>\<^sub>c x\<close>)
+
+also have "... = 
+(eval_func \<nat>\<^sub>c (\<nat>\<^sub>c \<times>\<^sub>c \<nat>\<^sub>c) \<circ>\<^sub>c 
+( id\<^sub>c (\<nat>\<^sub>c \<times>\<^sub>c \<nat>\<^sub>c) \<times>\<^sub>f
+(add2 \<circ>\<^sub>c
+\<langle>mult2 \<circ>\<^sub>c (left_cart_proj (\<nat>\<^sub>c\<times>\<^sub>c \<nat>\<^sub>c) (\<nat>\<^sub>c\<^bsup>(\<nat>\<^sub>c \<times>\<^sub>c \<nat>\<^sub>c)\<^esup>)   ) , 
+                             eval_func \<nat>\<^sub>c (\<nat>\<^sub>c \<times>\<^sub>c \<nat>\<^sub>c)   \<rangle>)\<^sup>\<sharp>
+ \<circ>\<^sub>cg)) \<circ>\<^sub>c x"
+  using g_def identity_distributes_across_composition multIdxMultp0p0p1p0p1_Sharp_type by (typecheck_cfuncs, auto)
+
+  also have "... =  (eval_func \<nat>\<^sub>c (\<nat>\<^sub>c \<times>\<^sub>c \<nat>\<^sub>c) \<circ>\<^sub>c id\<^sub>c (\<nat>\<^sub>c \<times>\<^sub>c \<nat>\<^sub>c) \<times>\<^sub>f (add2 \<circ>\<^sub>c \<langle>mult2 \<circ>\<^sub>c left_cart_proj (\<nat>\<^sub>c \<times>\<^sub>c \<nat>\<^sub>c) (\<nat>\<^sub>c\<^bsup>(\<nat>\<^sub>c \<times>\<^sub>c \<nat>\<^sub>c)\<^esup>),eval_func \<nat>\<^sub>c (\<nat>\<^sub>c \<times>\<^sub>c \<nat>\<^sub>c)\<rangle>)\<^sup>\<sharp> \<circ>\<^sub>c (mult2 \<circ>\<^sub>c (id\<^sub>c \<nat>\<^sub>c \<times>\<^sub>f mult2) \<circ>\<^sub>c \<langle>left_cart_proj \<nat>\<^sub>c \<nat>\<^sub>c \<circ>\<^sub>c left_cart_proj (\<nat>\<^sub>c \<times>\<^sub>c \<nat>\<^sub>c) \<nat>\<^sub>c,\<langle>right_cart_proj \<nat>\<^sub>c \<nat>\<^sub>c \<circ>\<^sub>c left_cart_proj (\<nat>\<^sub>c \<times>\<^sub>c \<nat>\<^sub>c) \<nat>\<^sub>c,right_cart_proj (\<nat>\<^sub>c \<times>\<^sub>c \<nat>\<^sub>c) \<nat>\<^sub>c\<rangle>\<rangle>)\<^sup>\<sharp>) \<circ>\<^sub>c x "
+    using g_def by blast
+
+  then show  "(eval_func \<nat>\<^sub>c (\<nat>\<^sub>c \<times>\<^sub>c \<nat>\<^sub>c) \<circ>\<^sub>c id\<^sub>c (\<nat>\<^sub>c \<times>\<^sub>c \<nat>\<^sub>c) \<times>\<^sub>f (mult2 \<circ>\<^sub>c (id\<^sub>c \<nat>\<^sub>c \<times>\<^sub>f mult2) \<circ>\<^sub>c \<langle>left_cart_proj \<nat>\<^sub>c \<nat>\<^sub>c \<circ>\<^sub>c left_cart_proj (\<nat>\<^sub>c \<times>\<^sub>c \<nat>\<^sub>c) \<nat>\<^sub>c,\<langle>right_cart_proj \<nat>\<^sub>c \<nat>\<^sub>c \<circ>\<^sub>c left_cart_proj (\<nat>\<^sub>c \<times>\<^sub>c \<nat>\<^sub>c) \<nat>\<^sub>c,right_cart_proj (\<nat>\<^sub>c \<times>\<^sub>c \<nat>\<^sub>c) \<nat>\<^sub>c\<rangle>\<rangle>)\<^sup>\<sharp> \<circ>\<^sub>c successor) \<circ>\<^sub>c x =
+ (eval_func \<nat>\<^sub>c (\<nat>\<^sub>c \<times>\<^sub>c \<nat>\<^sub>c) \<circ>\<^sub>c id\<^sub>c (\<nat>\<^sub>c \<times>\<^sub>c \<nat>\<^sub>c) \<times>\<^sub>f (add2 \<circ>\<^sub>c \<langle>mult2 \<circ>\<^sub>c left_cart_proj (\<nat>\<^sub>c \<times>\<^sub>c \<nat>\<^sub>c) (\<nat>\<^sub>c\<^bsup>(\<nat>\<^sub>c \<times>\<^sub>c \<nat>\<^sub>c)\<^esup>),eval_func \<nat>\<^sub>c (\<nat>\<^sub>c \<times>\<^sub>c \<nat>\<^sub>c)\<rangle>)\<^sup>\<sharp> \<circ>\<^sub>c (mult2 \<circ>\<^sub>c (id\<^sub>c \<nat>\<^sub>c \<times>\<^sub>f mult2) \<circ>\<^sub>c \<langle>left_cart_proj \<nat>\<^sub>c \<nat>\<^sub>c \<circ>\<^sub>c left_cart_proj (\<nat>\<^sub>c \<times>\<^sub>c \<nat>\<^sub>c) \<nat>\<^sub>c,\<langle>right_cart_proj \<nat>\<^sub>c \<nat>\<^sub>c \<circ>\<^sub>c left_cart_proj (\<nat>\<^sub>c \<times>\<^sub>c \<nat>\<^sub>c) \<nat>\<^sub>c,right_cart_proj (\<nat>\<^sub>c \<times>\<^sub>c \<nat>\<^sub>c) \<nat>\<^sub>c\<rangle>\<rangle>)\<^sup>\<sharp>) \<circ>\<^sub>c x "
+    by (simp add: calculation)
+qed
+qed
+qed
 qed
 
-(*Now we compute this pair... *)
+  have main_result_flat: "mult2 \<circ>\<^sub>c mult2 \<times>\<^sub>f id\<^sub>c \<nat>\<^sub>c =
+       mult2 \<circ>\<^sub>c (id\<^sub>c \<nat>\<^sub>c \<times>\<^sub>f mult2) \<circ>\<^sub>c \<langle>left_cart_proj \<nat>\<^sub>c \<nat>\<^sub>c \<circ>\<^sub>c left_cart_proj (\<nat>\<^sub>c \<times>\<^sub>c \<nat>\<^sub>c) \<nat>\<^sub>c,\<langle>right_cart_proj \<nat>\<^sub>c \<nat>\<^sub>c \<circ>\<^sub>c left_cart_proj (\<nat>\<^sub>c \<times>\<^sub>c \<nat>\<^sub>c) \<nat>\<^sub>c,right_cart_proj (\<nat>\<^sub>c \<times>\<^sub>c \<nat>\<^sub>c) \<nat>\<^sub>c\<rangle>\<rangle>"
+    by (metis flat_cancels_sharp main_result multIdxMultp0p0p1p0p1_type multmultId_type)
 
-  have f6: "((eval_func \<nat>\<^sub>c (\<nat>\<^sub>c\<times>\<^sub>c\<nat>\<^sub>c))\<circ>\<^sub>c 
-(id\<^sub>c (\<nat>\<^sub>c\<times>\<^sub>c\<nat>\<^sub>c) \<times>\<^sub>f ((add2 \<circ>\<^sub>c \<langle>mult2 \<circ>\<^sub>c (left_cart_proj (\<nat>\<^sub>c\<times>\<^sub>c\<nat>\<^sub>c) (\<nat>\<^sub>c\<^bsup>(\<nat>\<^sub>c\<times>\<^sub>c\<nat>\<^sub>c)\<^esup>)),eval_func \<nat>\<^sub>c (\<nat>\<^sub>c\<times>\<^sub>c\<nat>\<^sub>c)\<rangle>)\<^sup>\<sharp>)
-\<circ>\<^sub>c ((mult2 \<circ>\<^sub>c (mult2 \<times>\<^sub>f id\<^sub>c \<nat>\<^sub>c))\<^sup>\<sharp>)
-))  \<circ>\<^sub>c \<langle>\<langle>a,b\<rangle>,c\<rangle> = (a \<cdot>\<^sub>\<nat> b)  \<cdot>\<^sub>\<nat> (successor  \<circ>\<^sub>c c)"
-  proof - 
-    have "((eval_func \<nat>\<^sub>c (\<nat>\<^sub>c\<times>\<^sub>c\<nat>\<^sub>c))\<circ>\<^sub>c 
-(id\<^sub>c (\<nat>\<^sub>c\<times>\<^sub>c\<nat>\<^sub>c) \<times>\<^sub>f ((add2 \<circ>\<^sub>c \<langle>mult2 \<circ>\<^sub>c (left_cart_proj (\<nat>\<^sub>c\<times>\<^sub>c\<nat>\<^sub>c) (\<nat>\<^sub>c\<^bsup>(\<nat>\<^sub>c\<times>\<^sub>c\<nat>\<^sub>c)\<^esup>)),eval_func \<nat>\<^sub>c (\<nat>\<^sub>c\<times>\<^sub>c\<nat>\<^sub>c)\<rangle>)\<^sup>\<sharp>)
-\<circ>\<^sub>c ((mult2 \<circ>\<^sub>c (mult2 \<times>\<^sub>f id\<^sub>c \<nat>\<^sub>c))\<^sup>\<sharp>)
-))  \<circ>\<^sub>c \<langle>\<langle>a,b\<rangle>,c\<rangle> = 
- (eval_func \<nat>\<^sub>c (\<nat>\<^sub>c\<times>\<^sub>c\<nat>\<^sub>c))\<circ>\<^sub>c 
-(id\<^sub>c (\<nat>\<^sub>c\<times>\<^sub>c\<nat>\<^sub>c) \<times>\<^sub>f ((add2 \<circ>\<^sub>c \<langle>mult2 \<circ>\<^sub>c (left_cart_proj (\<nat>\<^sub>c\<times>\<^sub>c\<nat>\<^sub>c) (\<nat>\<^sub>c\<^bsup>(\<nat>\<^sub>c\<times>\<^sub>c\<nat>\<^sub>c)\<^esup>)),eval_func \<nat>\<^sub>c (\<nat>\<^sub>c\<times>\<^sub>c\<nat>\<^sub>c)\<rangle>)\<^sup>\<sharp>)
-\<circ>\<^sub>c ((mult2 \<circ>\<^sub>c (mult2 \<times>\<^sub>f id\<^sub>c \<nat>\<^sub>c))\<^sup>\<sharp>)
-)  \<circ>\<^sub>c \<langle>\<langle>a,b\<rangle>,c\<rangle>"
-          using assms by (typecheck_cfuncs, simp add: comp_associative2)
-    also have "... = (eval_func \<nat>\<^sub>c (\<nat>\<^sub>c\<times>\<^sub>c\<nat>\<^sub>c))\<circ>\<^sub>c 
-(id\<^sub>c (\<nat>\<^sub>c\<times>\<^sub>c\<nat>\<^sub>c) \<times>\<^sub>f ((add2 \<circ>\<^sub>c \<langle>mult2 \<circ>\<^sub>c (left_cart_proj (\<nat>\<^sub>c\<times>\<^sub>c\<nat>\<^sub>c) (\<nat>\<^sub>c\<^bsup>(\<nat>\<^sub>c\<times>\<^sub>c\<nat>\<^sub>c)\<^esup>)),eval_func \<nat>\<^sub>c (\<nat>\<^sub>c\<times>\<^sub>c\<nat>\<^sub>c)\<rangle>)\<^sup>\<sharp>)) \<circ>\<^sub>c 
-(id\<^sub>c (\<nat>\<^sub>c\<times>\<^sub>c\<nat>\<^sub>c) \<times>\<^sub>f ((mult2 \<circ>\<^sub>c (mult2 \<times>\<^sub>f id\<^sub>c \<nat>\<^sub>c))\<^sup>\<sharp>))\<circ>\<^sub>c
-\<langle>\<langle>a,b\<rangle>,c\<rangle>"
-          using assms by (typecheck_cfuncs, smt comp_associative2 inv_transpose_func_def2 inv_transpose_of_composition transpose_func_def)
-    also have "... = (add2 \<circ>\<^sub>c \<langle>mult2 \<circ>\<^sub>c (left_cart_proj (\<nat>\<^sub>c\<times>\<^sub>c\<nat>\<^sub>c) (\<nat>\<^sub>c\<^bsup>(\<nat>\<^sub>c\<times>\<^sub>c\<nat>\<^sub>c)\<^esup>)),eval_func \<nat>\<^sub>c (\<nat>\<^sub>c\<times>\<^sub>c\<nat>\<^sub>c)\<rangle>) \<circ>\<^sub>c 
-(id\<^sub>c (\<nat>\<^sub>c\<times>\<^sub>c\<nat>\<^sub>c) \<times>\<^sub>f ((mult2 \<circ>\<^sub>c (mult2 \<times>\<^sub>f id\<^sub>c \<nat>\<^sub>c))\<^sup>\<sharp>))\<circ>\<^sub>c
-\<langle>\<langle>a,b\<rangle>,c\<rangle>"
-          using assms by (typecheck_cfuncs, smt comp_associative2 transpose_func_def)
-    also have "... = ((add2 \<circ>\<^sub>c
-\<langle>mult2 \<circ>\<^sub>c (left_cart_proj (\<nat>\<^sub>c\<times>\<^sub>c\<nat>\<^sub>c) (\<nat>\<^sub>c\<^bsup>(\<nat>\<^sub>c\<times>\<^sub>c\<nat>\<^sub>c)\<^esup>)),
-eval_func \<nat>\<^sub>c (\<nat>\<^sub>c\<times>\<^sub>c\<nat>\<^sub>c)\<rangle>) 
-\<circ>\<^sub>c (id\<^sub>c (\<nat>\<^sub>c\<times>\<^sub>c\<nat>\<^sub>c) \<times>\<^sub>f ((mult2 \<circ>\<^sub>c (mult2 \<times>\<^sub>f id\<^sub>c \<nat>\<^sub>c))\<^sup>\<sharp>)))
-\<circ>\<^sub>c\<langle>\<langle>a,b\<rangle>,c\<rangle>"
-                using assms by (typecheck_cfuncs, simp add: comp_associative2)
-    also have "... = (
-add2 \<circ>\<^sub>c
-\<langle>mult2 \<circ>\<^sub>c (left_cart_proj (\<nat>\<^sub>c\<times>\<^sub>c\<nat>\<^sub>c) (\<nat>\<^sub>c\<^bsup>(\<nat>\<^sub>c\<times>\<^sub>c\<nat>\<^sub>c)\<^esup>))
-\<circ>\<^sub>c (id\<^sub>c (\<nat>\<^sub>c\<times>\<^sub>c\<nat>\<^sub>c) \<times>\<^sub>f ((mult2 \<circ>\<^sub>c (mult2 \<times>\<^sub>f id\<^sub>c \<nat>\<^sub>c))\<^sup>\<sharp>)),
-eval_func \<nat>\<^sub>c (\<nat>\<^sub>c\<times>\<^sub>c\<nat>\<^sub>c)
-\<circ>\<^sub>c (id\<^sub>c (\<nat>\<^sub>c\<times>\<^sub>c\<nat>\<^sub>c) \<times>\<^sub>f ((mult2 \<circ>\<^sub>c (mult2 \<times>\<^sub>f id\<^sub>c \<nat>\<^sub>c))\<^sup>\<sharp>))\<rangle> 
-)
-\<circ>\<^sub>c\<langle>\<langle>a,b\<rangle>,c\<rangle>"
-          using assms by (typecheck_cfuncs, smt cfunc_prod_comp comp_associative2)
-    also have "... = (
-add2 \<circ>\<^sub>c
-\<langle>mult2 \<circ>\<^sub>c (id\<^sub>c (\<nat>\<^sub>c\<times>\<^sub>c\<nat>\<^sub>c) \<circ>\<^sub>c left_cart_proj (\<nat>\<^sub>c\<times>\<^sub>c\<nat>\<^sub>c) \<nat>\<^sub>c) ,
-eval_func \<nat>\<^sub>c (\<nat>\<^sub>c\<times>\<^sub>c\<nat>\<^sub>c)
-\<circ>\<^sub>c (id\<^sub>c (\<nat>\<^sub>c\<times>\<^sub>c\<nat>\<^sub>c) \<times>\<^sub>f ((mult2 \<circ>\<^sub>c (mult2 \<times>\<^sub>f id\<^sub>c \<nat>\<^sub>c))\<^sup>\<sharp>))\<rangle> 
-)
-\<circ>\<^sub>c\<langle>\<langle>a,b\<rangle>,c\<rangle>"
-          using assms by (typecheck_cfuncs, simp add: left_cart_proj_cfunc_cross_prod)
-    also have "... = 
-add2 \<circ>\<^sub>c
-\<langle>mult2 \<circ>\<^sub>c left_cart_proj (\<nat>\<^sub>c\<times>\<^sub>c\<nat>\<^sub>c) \<nat>\<^sub>c ,
-eval_func \<nat>\<^sub>c (\<nat>\<^sub>c\<times>\<^sub>c\<nat>\<^sub>c)
-\<circ>\<^sub>c (id\<^sub>c (\<nat>\<^sub>c\<times>\<^sub>c\<nat>\<^sub>c) \<times>\<^sub>f ((mult2 \<circ>\<^sub>c (mult2 \<times>\<^sub>f id\<^sub>c \<nat>\<^sub>c))\<^sup>\<sharp>))\<rangle> 
-\<circ>\<^sub>c\<langle>\<langle>a,b\<rangle>,c\<rangle>"
-          using assms by (typecheck_cfuncs, simp add: comp_associative2 id_left_unit2)
-also have "... = add2 \<circ>\<^sub>c
-\<langle>mult2 \<circ>\<^sub>c left_cart_proj (\<nat>\<^sub>c\<times>\<^sub>c\<nat>\<^sub>c) \<nat>\<^sub>c \<circ>\<^sub>c\<langle>\<langle>a,b\<rangle>,c\<rangle> ,
-eval_func \<nat>\<^sub>c (\<nat>\<^sub>c\<times>\<^sub>c\<nat>\<^sub>c)
-\<circ>\<^sub>c (id\<^sub>c (\<nat>\<^sub>c\<times>\<^sub>c\<nat>\<^sub>c) \<times>\<^sub>f ((mult2 \<circ>\<^sub>c (mult2 \<times>\<^sub>f id\<^sub>c \<nat>\<^sub>c))\<^sup>\<sharp>))\<circ>\<^sub>c\<langle>\<langle>a,b\<rangle>,c\<rangle>   \<rangle>"
-         apply(subst cfunc_prod_comp[where X = "one", where Y= "(\<nat>\<^sub>c\<times>\<^sub>c\<nat>\<^sub>c)\<times>\<^sub>c\<nat>\<^sub>c",
-                    where A = "\<nat>\<^sub>c", where B= "\<nat>\<^sub>c"])
-          using abc_type apply force
-          using comp_type left_cart_proj_type mult2_type apply blast
-          using multmultId_type transpose_func_def apply auto[1]
-          using assms by (typecheck_cfuncs, simp add: comp_associative2)
-
-also have "... =  add2 \<circ>\<^sub>c\<langle>mult2 \<circ>\<^sub>c  \<langle>a,b\<rangle> ,(mult2 \<circ>\<^sub>c (mult2 \<times>\<^sub>f id\<^sub>c \<nat>\<^sub>c)) \<circ>\<^sub>c\<langle>\<langle>a,b\<rangle>,c\<rangle>   \<rangle>"
-          using assms by (typecheck_cfuncs, simp add: comp_associative2 left_cart_proj_cfunc_prod transpose_func_def)
-  also have "... = add2 \<circ>\<^sub>c\<langle>mult2 \<circ>\<^sub>c  \<langle>a,b\<rangle> ,mult2  \<circ>\<^sub>c\<langle>mult2 \<circ>\<^sub>c\<langle>a,b\<rangle>,id\<^sub>c \<nat>\<^sub>c \<circ>\<^sub>c c\<rangle>   \<rangle>"
-          using assms by (typecheck_cfuncs, smt cfunc_cross_prod_comp_cfunc_prod comp_associative2)
-  also have "... = (a \<cdot>\<^sub>\<nat> b) +\<^sub>\<nat> ((a \<cdot>\<^sub>\<nat> b)\<cdot>\<^sub>\<nat> c)"
-    using add_def assms(3) id_left_unit2 mult_def by auto
-  also have "... =  (a \<cdot>\<^sub>\<nat> b)  \<cdot>\<^sub>\<nat> (successor  \<circ>\<^sub>c c)"
-    using assms(3) mult_def mult_respects_succ_right multab_type by auto
-then show ?thesis using calculation by auto
+  have ab_type: "\<langle>a,b\<rangle> \<in>\<^sub>c (\<nat>\<^sub>c \<times>\<^sub>c \<nat>\<^sub>c)"
+    by (simp add: assms(1) assms(2) cfunc_prod_type)
+  have bc_type: "\<langle>b ,c \<rangle> \<in>\<^sub>c (\<nat>\<^sub>c \<times>\<^sub>c \<nat>\<^sub>c)"
+    by (simp add: assms(2) assms(3) cfunc_prod_type)
+  have abc_type: "\<langle>\<langle>a,b\<rangle>,c\<rangle> \<in>\<^sub>c (\<nat>\<^sub>c \<times>\<^sub>c \<nat>\<^sub>c)\<times>\<^sub>c \<nat>\<^sub>c"
+    by (simp add: ab_type assms(3) cfunc_prod_type)
+  have result: "(a \<cdot>\<^sub>\<nat>  b) \<cdot>\<^sub>\<nat> c = mult2 \<circ>\<^sub>c \<langle> (a \<cdot>\<^sub>\<nat>  b), c\<rangle>"
+    by (simp add: mult_def)
+  also have "... = mult2 \<circ>\<^sub>c \<langle> mult2 \<circ>\<^sub>c \<langle>a,b\<rangle>,id\<^sub>c \<nat>\<^sub>c \<circ>\<^sub>c c\<rangle>"
+    using assms(3) id_left_unit2 mult_def by auto
+  also have "... = mult2 \<circ>\<^sub>c (mult2 \<times>\<^sub>f id\<^sub>c \<nat>\<^sub>c) \<circ>\<^sub>c \<langle>  \<langle>a,b\<rangle>, c\<rangle>"
+    using ab_type assms(3) cfunc_cross_prod_comp_cfunc_prod by (typecheck_cfuncs,auto)
+  also have "... = (mult2 \<circ>\<^sub>c (mult2 \<times>\<^sub>f id\<^sub>c \<nat>\<^sub>c)) \<circ>\<^sub>c \<langle>  \<langle>a,b\<rangle>, c\<rangle>"
+    using abc_type comp_associative2 by (typecheck_cfuncs, auto)  
+  also have "... =  mult2 \<circ>\<^sub>c (id\<^sub>c \<nat>\<^sub>c \<times>\<^sub>f mult2) \<circ>\<^sub>c \<langle>left_cart_proj \<nat>\<^sub>c \<nat>\<^sub>c \<circ>\<^sub>c left_cart_proj (\<nat>\<^sub>c \<times>\<^sub>c \<nat>\<^sub>c) \<nat>\<^sub>c,\<langle>right_cart_proj \<nat>\<^sub>c \<nat>\<^sub>c \<circ>\<^sub>c left_cart_proj (\<nat>\<^sub>c \<times>\<^sub>c \<nat>\<^sub>c) \<nat>\<^sub>c,right_cart_proj (\<nat>\<^sub>c \<times>\<^sub>c \<nat>\<^sub>c) \<nat>\<^sub>c\<rangle>\<rangle>
+                    \<circ>\<^sub>c \<langle>  \<langle>a,b\<rangle>, c\<rangle>"
+    by (typecheck_cfuncs, smt abc_type cfunc_type_def comp_associative domain_comp main_result_flat)
+  also have "... =  mult2 \<circ>\<^sub>c (id\<^sub>c \<nat>\<^sub>c \<times>\<^sub>f mult2) \<circ>\<^sub>c \<langle>left_cart_proj \<nat>\<^sub>c \<nat>\<^sub>c \<circ>\<^sub>c left_cart_proj (\<nat>\<^sub>c \<times>\<^sub>c \<nat>\<^sub>c) \<nat>\<^sub>c \<circ>\<^sub>c \<langle>  \<langle>a,b\<rangle>, c\<rangle> ,\<langle>right_cart_proj \<nat>\<^sub>c \<nat>\<^sub>c \<circ>\<^sub>c left_cart_proj (\<nat>\<^sub>c \<times>\<^sub>c \<nat>\<^sub>c) \<nat>\<^sub>c \<circ>\<^sub>c \<langle>  \<langle>a,b\<rangle>, c\<rangle> ,right_cart_proj (\<nat>\<^sub>c \<times>\<^sub>c \<nat>\<^sub>c) \<nat>\<^sub>c \<circ>\<^sub>c \<langle>  \<langle>a,b\<rangle>, c\<rangle> \<rangle> \<rangle>"
+    using abc_type cfunc_prod_comp comp_associative2 by (typecheck_cfuncs, auto)
+  also have "... =  mult2 \<circ>\<^sub>c (id\<^sub>c \<nat>\<^sub>c \<times>\<^sub>f mult2) \<circ>\<^sub>c \<langle>a ,\<langle>b ,c \<rangle> \<rangle>"
+    by (typecheck_cfuncs, smt assms left_cart_proj_cfunc_prod right_cart_proj_cfunc_prod)
+  also have "... =  mult2 \<circ>\<^sub>c \<langle>id\<^sub>c \<nat>\<^sub>c \<circ>\<^sub>c  a ,mult2 \<circ>\<^sub>c \<langle>b ,c \<rangle> \<rangle>"
+    using assms(1) bc_type cfunc_cross_prod_comp_cfunc_prod by (typecheck_cfuncs, auto)
+  also have "... =  mult2 \<circ>\<^sub>c \<langle>a , b \<cdot>\<^sub>\<nat> c  \<rangle>"
+    using assms(1) id_left_unit2 mult_def by auto
+  also have "... = a \<cdot>\<^sub>\<nat> (b \<cdot>\<^sub>\<nat> c )"
+    by (simp add: mult_def)
+  then show ?thesis using calculation by auto
 qed
 
 
-(*Next to last on page 20*)
-
-
-
-  have f7: "((eval_func \<nat>\<^sub>c (\<nat>\<^sub>c\<times>\<^sub>c\<nat>\<^sub>c))\<circ>\<^sub>c 
-(id\<^sub>c (\<nat>\<^sub>c\<times>\<^sub>c\<nat>\<^sub>c) \<times>\<^sub>f ((add2 \<circ>\<^sub>c \<langle>mult2 \<circ>\<^sub>c (left_cart_proj (\<nat>\<^sub>c\<times>\<^sub>c\<nat>\<^sub>c) (\<nat>\<^sub>c\<^bsup>(\<nat>\<^sub>c\<times>\<^sub>c\<nat>\<^sub>c)\<^esup>)),eval_func \<nat>\<^sub>c (\<nat>\<^sub>c\<times>\<^sub>c\<nat>\<^sub>c)\<rangle>)\<^sup>\<sharp>)
-\<circ>\<^sub>c  (mult2 \<circ>\<^sub>c (id\<^sub>c \<nat>\<^sub>c  \<times>\<^sub>f mult2) \<circ>\<^sub>c \<langle>(left_cart_proj \<nat>\<^sub>c \<nat>\<^sub>c) \<circ>\<^sub>c (left_cart_proj (\<nat>\<^sub>c\<times>\<^sub>c \<nat>\<^sub>c) \<nat>\<^sub>c),
-\<langle>(right_cart_proj \<nat>\<^sub>c \<nat>\<^sub>c) \<circ>\<^sub>c (left_cart_proj (\<nat>\<^sub>c\<times>\<^sub>c \<nat>\<^sub>c) \<nat>\<^sub>c), (right_cart_proj (\<nat>\<^sub>c\<times>\<^sub>c \<nat>\<^sub>c) \<nat>\<^sub>c)\<rangle>\<rangle>)\<^sup>\<sharp>
-))  \<circ>\<^sub>c \<langle>\<langle>a,b\<rangle>,c\<rangle> = a \<cdot>\<^sub>\<nat> (b  \<cdot>\<^sub>\<nat> (successor  \<circ>\<^sub>c c))"
-  proof - 
-    have "((eval_func \<nat>\<^sub>c (\<nat>\<^sub>c\<times>\<^sub>c\<nat>\<^sub>c))\<circ>\<^sub>c 
-(id\<^sub>c (\<nat>\<^sub>c\<times>\<^sub>c\<nat>\<^sub>c) \<times>\<^sub>f ((add2 \<circ>\<^sub>c \<langle>mult2 \<circ>\<^sub>c (left_cart_proj (\<nat>\<^sub>c\<times>\<^sub>c\<nat>\<^sub>c) (\<nat>\<^sub>c\<^bsup>(\<nat>\<^sub>c\<times>\<^sub>c\<nat>\<^sub>c)\<^esup>)),eval_func \<nat>\<^sub>c (\<nat>\<^sub>c\<times>\<^sub>c\<nat>\<^sub>c)\<rangle>)\<^sup>\<sharp>)
-\<circ>\<^sub>c  (mult2 \<circ>\<^sub>c (id\<^sub>c \<nat>\<^sub>c  \<times>\<^sub>f mult2) \<circ>\<^sub>c \<langle>(left_cart_proj \<nat>\<^sub>c \<nat>\<^sub>c) \<circ>\<^sub>c (left_cart_proj (\<nat>\<^sub>c\<times>\<^sub>c \<nat>\<^sub>c) \<nat>\<^sub>c),
-\<langle>(right_cart_proj \<nat>\<^sub>c \<nat>\<^sub>c) \<circ>\<^sub>c (left_cart_proj (\<nat>\<^sub>c\<times>\<^sub>c \<nat>\<^sub>c) \<nat>\<^sub>c), (right_cart_proj (\<nat>\<^sub>c\<times>\<^sub>c \<nat>\<^sub>c) \<nat>\<^sub>c)\<rangle>\<rangle>)\<^sup>\<sharp>
-))  \<circ>\<^sub>c \<langle>\<langle>a,b\<rangle>,c\<rangle> =   
-((eval_func \<nat>\<^sub>c (\<nat>\<^sub>c\<times>\<^sub>c\<nat>\<^sub>c))\<circ>\<^sub>c 
-(id\<^sub>c (\<nat>\<^sub>c\<times>\<^sub>c\<nat>\<^sub>c) \<times>\<^sub>f ((add2 \<circ>\<^sub>c \<langle>mult2 \<circ>\<^sub>c (left_cart_proj (\<nat>\<^sub>c\<times>\<^sub>c\<nat>\<^sub>c) (\<nat>\<^sub>c\<^bsup>(\<nat>\<^sub>c\<times>\<^sub>c\<nat>\<^sub>c)\<^esup>)),eval_func \<nat>\<^sub>c (\<nat>\<^sub>c\<times>\<^sub>c\<nat>\<^sub>c)\<rangle>)\<^sup>\<sharp>)
-))
-\<circ>\<^sub>c ( id\<^sub>c (\<nat>\<^sub>c\<times>\<^sub>c\<nat>\<^sub>c) \<times>\<^sub>f  (mult2 \<circ>\<^sub>c (id\<^sub>c \<nat>\<^sub>c  \<times>\<^sub>f mult2) \<circ>\<^sub>c \<langle>(left_cart_proj \<nat>\<^sub>c \<nat>\<^sub>c) \<circ>\<^sub>c (left_cart_proj (\<nat>\<^sub>c\<times>\<^sub>c \<nat>\<^sub>c) \<nat>\<^sub>c),
-\<langle>(right_cart_proj \<nat>\<^sub>c \<nat>\<^sub>c) \<circ>\<^sub>c (left_cart_proj (\<nat>\<^sub>c\<times>\<^sub>c \<nat>\<^sub>c) \<nat>\<^sub>c), (right_cart_proj (\<nat>\<^sub>c\<times>\<^sub>c \<nat>\<^sub>c) \<nat>\<^sub>c)\<rangle>\<rangle>)\<^sup>\<sharp>)
-\<circ>\<^sub>c \<langle>\<langle>a,b\<rangle>,c\<rangle>"
-          using assms by (typecheck_cfuncs, smt comp_associative2 inv_transpose_func_def2 inv_transpose_of_composition)
-    also have "... = add2 \<circ>\<^sub>c \<langle>mult2 \<circ>\<^sub>c (left_cart_proj (\<nat>\<^sub>c\<times>\<^sub>c\<nat>\<^sub>c) (\<nat>\<^sub>c\<^bsup>(\<nat>\<^sub>c\<times>\<^sub>c\<nat>\<^sub>c)\<^esup>))
-, eval_func \<nat>\<^sub>c (\<nat>\<^sub>c\<times>\<^sub>c\<nat>\<^sub>c)
-\<rangle>
-\<circ>\<^sub>c ( id\<^sub>c (\<nat>\<^sub>c\<times>\<^sub>c\<nat>\<^sub>c) \<times>\<^sub>f  (mult2 \<circ>\<^sub>c (id\<^sub>c \<nat>\<^sub>c  \<times>\<^sub>f mult2) \<circ>\<^sub>c \<langle>(left_cart_proj \<nat>\<^sub>c \<nat>\<^sub>c) \<circ>\<^sub>c (left_cart_proj (\<nat>\<^sub>c\<times>\<^sub>c \<nat>\<^sub>c) \<nat>\<^sub>c),
-\<langle>(right_cart_proj \<nat>\<^sub>c \<nat>\<^sub>c) \<circ>\<^sub>c (left_cart_proj (\<nat>\<^sub>c\<times>\<^sub>c \<nat>\<^sub>c) \<nat>\<^sub>c), (right_cart_proj (\<nat>\<^sub>c\<times>\<^sub>c \<nat>\<^sub>c) \<nat>\<^sub>c)\<rangle>\<rangle>)\<^sup>\<sharp>)
-\<circ>\<^sub>c \<langle>\<langle>a,b\<rangle>,c\<rangle>"
-          using assms by (typecheck_cfuncs, smt cfunc_type_def comp_associative transpose_func_def)
-    also have "...  = (add2 \<circ>\<^sub>c \<langle>mult2 \<circ>\<^sub>c (left_cart_proj (\<nat>\<^sub>c\<times>\<^sub>c\<nat>\<^sub>c) (\<nat>\<^sub>c\<^bsup>(\<nat>\<^sub>c\<times>\<^sub>c\<nat>\<^sub>c)\<^esup>))
-, eval_func \<nat>\<^sub>c (\<nat>\<^sub>c\<times>\<^sub>c\<nat>\<^sub>c)
-\<rangle>
-\<circ>\<^sub>c ( id\<^sub>c (\<nat>\<^sub>c\<times>\<^sub>c\<nat>\<^sub>c) \<times>\<^sub>f  (mult2 \<circ>\<^sub>c (id\<^sub>c \<nat>\<^sub>c  \<times>\<^sub>f mult2) \<circ>\<^sub>c \<langle>(left_cart_proj \<nat>\<^sub>c \<nat>\<^sub>c) \<circ>\<^sub>c (left_cart_proj (\<nat>\<^sub>c\<times>\<^sub>c \<nat>\<^sub>c) \<nat>\<^sub>c),
-\<langle>(right_cart_proj \<nat>\<^sub>c \<nat>\<^sub>c) \<circ>\<^sub>c (left_cart_proj (\<nat>\<^sub>c\<times>\<^sub>c \<nat>\<^sub>c) \<nat>\<^sub>c), (right_cart_proj (\<nat>\<^sub>c\<times>\<^sub>c \<nat>\<^sub>c) \<nat>\<^sub>c)\<rangle>\<rangle>)\<^sup>\<sharp>)
-)\<circ>\<^sub>c \<langle>\<langle>a,b\<rangle>,c\<rangle>"
-      using assms apply typecheck_cfuncs
-      using comp_associative2 by auto
-    also have "... = (add2 \<circ>\<^sub>c \<langle>mult2 \<circ>\<^sub>c (left_cart_proj (\<nat>\<^sub>c\<times>\<^sub>c\<nat>\<^sub>c) (\<nat>\<^sub>c\<^bsup>(\<nat>\<^sub>c\<times>\<^sub>c\<nat>\<^sub>c)\<^esup>))
-\<circ>\<^sub>c ( id\<^sub>c (\<nat>\<^sub>c\<times>\<^sub>c\<nat>\<^sub>c) \<times>\<^sub>f  (mult2 \<circ>\<^sub>c (id\<^sub>c \<nat>\<^sub>c  \<times>\<^sub>f mult2) \<circ>\<^sub>c \<langle>(left_cart_proj \<nat>\<^sub>c \<nat>\<^sub>c) \<circ>\<^sub>c (left_cart_proj (\<nat>\<^sub>c\<times>\<^sub>c \<nat>\<^sub>c) \<nat>\<^sub>c),
-\<langle>(right_cart_proj \<nat>\<^sub>c \<nat>\<^sub>c) \<circ>\<^sub>c (left_cart_proj (\<nat>\<^sub>c\<times>\<^sub>c \<nat>\<^sub>c) \<nat>\<^sub>c), (right_cart_proj (\<nat>\<^sub>c\<times>\<^sub>c \<nat>\<^sub>c) \<nat>\<^sub>c)\<rangle>\<rangle>)\<^sup>\<sharp>)
-, eval_func \<nat>\<^sub>c (\<nat>\<^sub>c\<times>\<^sub>c\<nat>\<^sub>c)
-\<circ>\<^sub>c ( id\<^sub>c (\<nat>\<^sub>c\<times>\<^sub>c\<nat>\<^sub>c) \<times>\<^sub>f  (mult2 \<circ>\<^sub>c (id\<^sub>c \<nat>\<^sub>c  \<times>\<^sub>f mult2) \<circ>\<^sub>c \<langle>(left_cart_proj \<nat>\<^sub>c \<nat>\<^sub>c) \<circ>\<^sub>c (left_cart_proj (\<nat>\<^sub>c\<times>\<^sub>c \<nat>\<^sub>c) \<nat>\<^sub>c),
-\<langle>(right_cart_proj \<nat>\<^sub>c \<nat>\<^sub>c) \<circ>\<^sub>c (left_cart_proj (\<nat>\<^sub>c\<times>\<^sub>c \<nat>\<^sub>c) \<nat>\<^sub>c), (right_cart_proj (\<nat>\<^sub>c\<times>\<^sub>c \<nat>\<^sub>c) \<nat>\<^sub>c)\<rangle>\<rangle>)\<^sup>\<sharp>)\<rangle>
-)\<circ>\<^sub>c \<langle>\<langle>a,b\<rangle>,c\<rangle>"
-      apply (subst cfunc_prod_comp[where X ="(\<nat>\<^sub>c\<times>\<^sub>c \<nat>\<^sub>c)\<times>\<^sub>c \<nat>\<^sub>c",
-          where Y = "(\<nat>\<^sub>c\<times>\<^sub>c \<nat>\<^sub>c)\<times>\<^sub>c(\<nat>\<^sub>c\<^bsup>(\<nat>\<^sub>c\<times>\<^sub>c\<nat>\<^sub>c)\<^esup>)", where A= "\<nat>\<^sub>c", where B="\<nat>\<^sub>c"])
-      apply (simp add: cfunc_cross_prod_type id_type multIdxMultp0p0p1p0p1_Sharp_type)
-      using multsigma0_type apply blast
-      using eval_func_type apply force
-      using assms by (typecheck_cfuncs, simp add: comp_associative2)
-    also have "... = (add2 \<circ>\<^sub>c \<langle>mult2 \<circ>\<^sub>c (left_cart_proj (\<nat>\<^sub>c\<times>\<^sub>c\<nat>\<^sub>c) (\<nat>\<^sub>c\<^bsup>(\<nat>\<^sub>c\<times>\<^sub>c\<nat>\<^sub>c)\<^esup>))
-\<circ>\<^sub>c ( id\<^sub>c (\<nat>\<^sub>c\<times>\<^sub>c\<nat>\<^sub>c) \<times>\<^sub>f  (mult2 \<circ>\<^sub>c (id\<^sub>c \<nat>\<^sub>c  \<times>\<^sub>f mult2) \<circ>\<^sub>c \<langle>(left_cart_proj \<nat>\<^sub>c \<nat>\<^sub>c) \<circ>\<^sub>c (left_cart_proj (\<nat>\<^sub>c\<times>\<^sub>c \<nat>\<^sub>c) \<nat>\<^sub>c),
-\<langle>(right_cart_proj \<nat>\<^sub>c \<nat>\<^sub>c) \<circ>\<^sub>c (left_cart_proj (\<nat>\<^sub>c\<times>\<^sub>c \<nat>\<^sub>c) \<nat>\<^sub>c), (right_cart_proj (\<nat>\<^sub>c\<times>\<^sub>c \<nat>\<^sub>c) \<nat>\<^sub>c)\<rangle>\<rangle>)\<^sup>\<sharp>)
-, 
-  mult2 \<circ>\<^sub>c (id\<^sub>c \<nat>\<^sub>c  \<times>\<^sub>f mult2) \<circ>\<^sub>c \<langle>(left_cart_proj \<nat>\<^sub>c \<nat>\<^sub>c) \<circ>\<^sub>c (left_cart_proj (\<nat>\<^sub>c\<times>\<^sub>c \<nat>\<^sub>c) \<nat>\<^sub>c),
-\<langle>(right_cart_proj \<nat>\<^sub>c \<nat>\<^sub>c) \<circ>\<^sub>c (left_cart_proj (\<nat>\<^sub>c\<times>\<^sub>c \<nat>\<^sub>c) \<nat>\<^sub>c), (right_cart_proj (\<nat>\<^sub>c\<times>\<^sub>c \<nat>\<^sub>c) \<nat>\<^sub>c)\<rangle>\<rangle>\<rangle>
-)\<circ>\<^sub>c \<langle>\<langle>a,b\<rangle>,c\<rangle>"
-      using multIdxMultp0p0p1p0p1_type transpose_func_def by auto
-    also have "... = 
-(add2 \<circ>\<^sub>c \<langle>mult2 \<circ>\<^sub>c (id\<^sub>c (\<nat>\<^sub>c\<times>\<^sub>c\<nat>\<^sub>c) \<circ>\<^sub>c left_cart_proj (\<nat>\<^sub>c\<times>\<^sub>c\<nat>\<^sub>c) \<nat>\<^sub>c)  
-, 
-  mult2 \<circ>\<^sub>c (id\<^sub>c \<nat>\<^sub>c  \<times>\<^sub>f mult2) \<circ>\<^sub>c \<langle>(left_cart_proj \<nat>\<^sub>c \<nat>\<^sub>c) \<circ>\<^sub>c (left_cart_proj (\<nat>\<^sub>c\<times>\<^sub>c \<nat>\<^sub>c) \<nat>\<^sub>c),
-\<langle>(right_cart_proj \<nat>\<^sub>c \<nat>\<^sub>c) \<circ>\<^sub>c (left_cart_proj (\<nat>\<^sub>c\<times>\<^sub>c \<nat>\<^sub>c) \<nat>\<^sub>c), (right_cart_proj (\<nat>\<^sub>c\<times>\<^sub>c \<nat>\<^sub>c) \<nat>\<^sub>c)\<rangle>\<rangle>\<rangle>
-)\<circ>\<^sub>c \<langle>\<langle>a,b\<rangle>,c\<rangle>"
-      by (smt id_type left_cart_proj_cfunc_cross_prod multIdxMultp0p0p1p0p1_Sharp_type)
-    also have "... = 
-     (add2 \<circ>\<^sub>c \<langle>mult2 \<circ>\<^sub>c (id\<^sub>c (\<nat>\<^sub>c\<times>\<^sub>c\<nat>\<^sub>c) \<circ>\<^sub>c left_cart_proj (\<nat>\<^sub>c\<times>\<^sub>c\<nat>\<^sub>c) \<nat>\<^sub>c)  
-, 
-  mult2  \<circ>\<^sub>c
- \<langle>id\<^sub>c \<nat>\<^sub>c \<circ>\<^sub>c  (left_cart_proj \<nat>\<^sub>c \<nat>\<^sub>c) \<circ>\<^sub>c (left_cart_proj (\<nat>\<^sub>c\<times>\<^sub>c \<nat>\<^sub>c) \<nat>\<^sub>c),
-mult2 \<circ>\<^sub>c \<langle>(right_cart_proj \<nat>\<^sub>c \<nat>\<^sub>c) \<circ>\<^sub>c (left_cart_proj (\<nat>\<^sub>c\<times>\<^sub>c \<nat>\<^sub>c) \<nat>\<^sub>c), (right_cart_proj (\<nat>\<^sub>c\<times>\<^sub>c \<nat>\<^sub>c) \<nat>\<^sub>c)\<rangle>
-\<rangle>
-\<rangle>
-)\<circ>\<^sub>c \<langle>\<langle>a,b\<rangle>,c\<rangle>"
-      using cfunc_cross_prod_comp_cfunc_prod id_type mult2_type p0rho0_type p1rho0rho1_type by fastforce
-    also have "... = add2 \<circ>\<^sub>c 
-\<langle>mult2 \<circ>\<^sub>c (left_cart_proj (\<nat>\<^sub>c\<times>\<^sub>c\<nat>\<^sub>c) \<nat>\<^sub>c)  
-, 
-  mult2  \<circ>\<^sub>c \<langle>(left_cart_proj \<nat>\<^sub>c \<nat>\<^sub>c) \<circ>\<^sub>c (left_cart_proj (\<nat>\<^sub>c\<times>\<^sub>c \<nat>\<^sub>c) \<nat>\<^sub>c),
-mult2 \<circ>\<^sub>c \<langle>(right_cart_proj \<nat>\<^sub>c \<nat>\<^sub>c) \<circ>\<^sub>c (left_cart_proj (\<nat>\<^sub>c\<times>\<^sub>c \<nat>\<^sub>c) \<nat>\<^sub>c), (right_cart_proj (\<nat>\<^sub>c\<times>\<^sub>c \<nat>\<^sub>c) \<nat>\<^sub>c)\<rangle>
-\<rangle>
-\<rangle>
-\<circ>\<^sub>c \<langle>\<langle>a,b\<rangle>,c\<rangle>"
-          using assms by (typecheck_cfuncs,simp add: comp_associative2 id_left_unit2)
-    also have "... = add2 \<circ>\<^sub>c 
-\<langle>mult2 \<circ>\<^sub>c (left_cart_proj (\<nat>\<^sub>c\<times>\<^sub>c\<nat>\<^sub>c) \<nat>\<^sub>c)  
-\<circ>\<^sub>c \<langle>\<langle>a,b\<rangle>,c\<rangle>
-,
-  mult2  \<circ>\<^sub>c \<langle>(left_cart_proj \<nat>\<^sub>c \<nat>\<^sub>c) \<circ>\<^sub>c (left_cart_proj (\<nat>\<^sub>c\<times>\<^sub>c \<nat>\<^sub>c) \<nat>\<^sub>c),
-mult2 \<circ>\<^sub>c \<langle>(right_cart_proj \<nat>\<^sub>c \<nat>\<^sub>c) \<circ>\<^sub>c (left_cart_proj (\<nat>\<^sub>c\<times>\<^sub>c \<nat>\<^sub>c) \<nat>\<^sub>c), (right_cart_proj (\<nat>\<^sub>c\<times>\<^sub>c \<nat>\<^sub>c) \<nat>\<^sub>c)\<rangle>
-\<rangle>
-\<circ>\<^sub>c \<langle>\<langle>a,b\<rangle>,c\<rangle> \<rangle>"
-      apply (subst cfunc_prod_comp[where X = "one", where Y = "(\<nat>\<^sub>c\<times>\<^sub>c \<nat>\<^sub>c)\<times>\<^sub>c\<nat>\<^sub>c",
-            where A = "\<nat>\<^sub>c", where B= "\<nat>\<^sub>c"])
-      using abc_type apply blast
-      using comp_type left_cart_proj_type mult2_type apply blast
-      apply (smt cfunc_cross_prod_comp_cfunc_prod id_left_unit2 id_type multIdxMultp0p0p1p0p1_type mult2_type p0rho0_type p1rho0rho1_type)
-      using assms by (typecheck_cfuncs, simp add: comp_associative2)
-
-    also have "... =add2 \<circ>\<^sub>c 
-\<langle>mult2 \<circ>\<^sub>c (left_cart_proj (\<nat>\<^sub>c\<times>\<^sub>c\<nat>\<^sub>c) \<nat>\<^sub>c)  
-\<circ>\<^sub>c \<langle>\<langle>a,b\<rangle>,c\<rangle>
-,
-  mult2  \<circ>\<^sub>c \<langle>(left_cart_proj \<nat>\<^sub>c \<nat>\<^sub>c) \<circ>\<^sub>c (left_cart_proj (\<nat>\<^sub>c\<times>\<^sub>c \<nat>\<^sub>c) \<nat>\<^sub>c) \<circ>\<^sub>c \<langle>\<langle>a,b\<rangle>,c\<rangle>
-,
-mult2 \<circ>\<^sub>c \<langle>(right_cart_proj \<nat>\<^sub>c \<nat>\<^sub>c) \<circ>\<^sub>c (left_cart_proj (\<nat>\<^sub>c\<times>\<^sub>c \<nat>\<^sub>c) \<nat>\<^sub>c), (right_cart_proj (\<nat>\<^sub>c\<times>\<^sub>c \<nat>\<^sub>c) \<nat>\<^sub>c)\<rangle>
-\<circ>\<^sub>c \<langle>\<langle>a,b\<rangle>,c\<rangle>
-\<rangle>
- \<rangle>"
-      apply (subst cfunc_prod_comp [where X = "one", where Y = "(\<nat>\<^sub>c\<times>\<^sub>c \<nat>\<^sub>c)\<times>\<^sub>c\<nat>\<^sub>c",
-            where  A = "\<nat>\<^sub>c", where B = "\<nat>\<^sub>c"])
-      using abc_type apply blast
-      using p0rho0_type apply fastforce
-      using comp_type mult2_type p1rho0rho1_type apply blast
-      using assms by (typecheck_cfuncs, simp add: comp_associative2)
-    also have "... = add2 \<circ>\<^sub>c 
-\<langle>mult2 \<circ>\<^sub>c (left_cart_proj (\<nat>\<^sub>c\<times>\<^sub>c\<nat>\<^sub>c) \<nat>\<^sub>c)  
-\<circ>\<^sub>c \<langle>\<langle>a,b\<rangle>,c\<rangle>
-,
-  mult2  \<circ>\<^sub>c \<langle>(left_cart_proj \<nat>\<^sub>c \<nat>\<^sub>c) \<circ>\<^sub>c (left_cart_proj (\<nat>\<^sub>c\<times>\<^sub>c \<nat>\<^sub>c) \<nat>\<^sub>c) \<circ>\<^sub>c \<langle>\<langle>a,b\<rangle>,c\<rangle>
-,
-mult2 \<circ>\<^sub>c \<langle>(right_cart_proj \<nat>\<^sub>c \<nat>\<^sub>c) \<circ>\<^sub>c (left_cart_proj (\<nat>\<^sub>c\<times>\<^sub>c \<nat>\<^sub>c) \<nat>\<^sub>c) \<circ>\<^sub>c \<langle>\<langle>a,b\<rangle>,c\<rangle>
-, (right_cart_proj (\<nat>\<^sub>c\<times>\<^sub>c \<nat>\<^sub>c) \<nat>\<^sub>c) \<circ>\<^sub>c \<langle>\<langle>a,b\<rangle>,c\<rangle>  \<rangle>
-\<rangle>
- \<rangle>"
-      using assms apply typecheck_cfuncs
-      using cfunc_prod_comp comp_associative2 by auto
-    also have "... = add2 \<circ>\<^sub>c
-\<langle>mult2 \<circ>\<^sub>c 
- \<langle>a,b\<rangle>
-,
-  mult2  \<circ>\<^sub>c \<langle>(left_cart_proj \<nat>\<^sub>c \<nat>\<^sub>c) \<circ>\<^sub>c \<langle>a,b\<rangle>
-,
-mult2 \<circ>\<^sub>c \<langle>(right_cart_proj \<nat>\<^sub>c \<nat>\<^sub>c) \<circ>\<^sub>c  \<langle>a,b\<rangle>
-, (right_cart_proj (\<nat>\<^sub>c\<times>\<^sub>c \<nat>\<^sub>c) \<nat>\<^sub>c) \<circ>\<^sub>c \<langle>\<langle>a,b\<rangle>,c\<rangle>  \<rangle>
-\<rangle>
- \<rangle>"
-      using ab_type assms(3) left_cart_proj_cfunc_prod by auto
-    also have "... = add2 \<circ>\<^sub>c 
-\<langle>mult2 \<circ>\<^sub>c \<langle>a,b\<rangle> ,mult2  \<circ>\<^sub>c \<langle>a, mult2 \<circ>\<^sub>c \<langle>b, c \<rangle>\<rangle>\<rangle>"
-      using ab_type assms left_cart_proj_cfunc_prod right_cart_proj_cfunc_prod by auto
-    also have "... =  (a \<cdot>\<^sub>\<nat> b) +\<^sub>\<nat> a \<cdot>\<^sub>\<nat> (b \<cdot>\<^sub>\<nat> c)"
-      by (simp add: add_def mult_def)
-    also have "... = a \<cdot>\<^sub>\<nat> b  +\<^sub>\<nat> (b \<cdot>\<^sub>\<nat> c) \<cdot>\<^sub>\<nat> a"
-
-HERE
-*)
-
-
-
-
-
-(* Don't forget to do Right Distributivity *)
 
 
 lemma mult_right_distributivity:
   assumes "a \<in>\<^sub>c  \<nat>\<^sub>c"  "b\<in>\<^sub>c  \<nat>\<^sub>c"  "c\<in>\<^sub>c  \<nat>\<^sub>c"
   shows "a \<cdot>\<^sub>\<nat> ( b +\<^sub>\<nat> c)   = (a \<cdot>\<^sub>\<nat> b) +\<^sub>\<nat>  (a \<cdot>\<^sub>\<nat> c)"
+  using add_type assms mult_Left_Distributivity mult_commutative by auto
+  
+
+lemma mult_cancellative:
+  assumes "a \<in>\<^sub>c \<nat>\<^sub>c" "b \<in>\<^sub>c \<nat>\<^sub>c" "c \<in>\<^sub>c \<nat>\<^sub>c" "c \<noteq> zero"
+  shows "(a \<cdot>\<^sub>\<nat> c = b \<cdot>\<^sub>\<nat> c) = (a = b)"
   oops
 
-lemma mult_pie_type: "mult2 \<circ>\<^sub>c\<langle>left_cart_proj \<nat>\<^sub>c (\<nat>\<^sub>c\<^bsup>\<nat>\<^sub>c\<^esup>),eval_func \<nat>\<^sub>c \<nat>\<^sub>c\<rangle>: \<nat>\<^sub>c \<times>\<^sub>c (\<nat>\<^sub>c\<^bsup>\<nat>\<^sub>c\<^esup>) \<rightarrow>  \<nat>\<^sub>c"
-  by (meson cfunc_prod_type comp_type eval_func_type left_cart_proj_type mult2_type)
-
-lemma mult_pie_sharp_type: "(mult2 \<circ>\<^sub>c\<langle>left_cart_proj \<nat>\<^sub>c (\<nat>\<^sub>c\<^bsup>\<nat>\<^sub>c\<^esup>),eval_func \<nat>\<^sub>c \<nat>\<^sub>c\<rangle>)\<^sup>\<sharp>: \<nat>\<^sub>c\<^bsup>\<nat>\<^sub>c\<^esup> \<rightarrow> \<nat>\<^sub>c\<^bsup>\<nat>\<^sub>c\<^esup>"
-  by (simp add: mult_pie_type transpose_func_type)
 
 end
